Edit (2026-07-12 02:58:32)

theories/A002/_appendix/_artifacts/A002_IO.ml
@@ -15,6 +15,12 @@ let fst = function
 let snd = function
 | (_, y) -> y
 
+(** val length : 'a1 list -> Big_int_Z.big_int **)
+
+let rec length = function
+| [] -> Big_int_Z.zero_big_int
+| _ :: l' -> Big_int_Z.succ_big_int (length l')
+
 (** val app : 'a1 list -> 'a1 list -> 'a1 list **)
 
 let rec app l m =
@@ -363,11 +369,6 @@ let reject stage index detail =
 let sTAGE_DERIVATION_HEADER =
   Big_int_Z.zero_big_int
 
-(** val sTAGE_LIST_STRUCTURE : Big_int_Z.big_int **)
-
-let sTAGE_LIST_STRUCTURE =
-  Big_int_Z.succ_big_int Big_int_Z.zero_big_int
-
 (** val sTAGE_LINE : Big_int_Z.big_int **)
 
 let sTAGE_LINE =
@@ -403,11 +404,6 @@ let sTAGE_CONCLUSION =
 let eRR_NONCANONICAL_DERIVATION =
   Big_int_Z.zero_big_int
 
-(** val eRR_BAD_DERIVATION_LENGTH : Big_int_Z.big_int **)
-
-let eRR_BAD_DERIVATION_LENGTH =
-  Big_int_Z.succ_big_int Big_int_Z.zero_big_int
-
 (** val eRR_EMPTY_DERIVATION : Big_int_Z.big_int **)
 
 let eRR_EMPTY_DERIVATION =
@@ -418,12 +414,6 @@ let eRR_EMPTY_DERIVATION =
 let eRR_BAD_CONCLUSION =
   Big_int_Z.succ_big_int (Big_int_Z.succ_big_int (Big_int_Z.succ_big_int
     Big_int_Z.zero_big_int))
-
-(** val eRR_FUEL_EXHAUSTED : Big_int_Z.big_int **)
-
-let eRR_FUEL_EXHAUSTED =
-  Big_int_Z.succ_big_int (Big_int_Z.succ_big_int (Big_int_Z.succ_big_int
-    (Big_int_Z.succ_big_int Big_int_Z.zero_big_int)))
 
 (** val eRR_NONCANONICAL_NODE : Big_int_Z.big_int **)
 
@@ -437,21 +427,6 @@ let eRR_BAD_TAG =
   Big_int_Z.succ_big_int (Big_int_Z.succ_big_int (Big_int_Z.succ_big_int
     (Big_int_Z.succ_big_int (Big_int_Z.succ_big_int (Big_int_Z.succ_big_int
     Big_int_Z.zero_big_int)))))
-
-(** val eRR_BAD_LIST_TAG : Big_int_Z.big_int **)
-
-let eRR_BAD_LIST_TAG =
-  Big_int_Z.succ_big_int (Big_int_Z.succ_big_int (Big_int_Z.succ_big_int
-    (Big_int_Z.succ_big_int (Big_int_Z.succ_big_int (Big_int_Z.succ_big_int
-    (Big_int_Z.succ_big_int Big_int_Z.zero_big_int))))))
-
-(** val eRR_INDEX_OUT_OF_RANGE : Big_int_Z.big_int **)
-
-let eRR_INDEX_OUT_OF_RANGE =
-  Big_int_Z.succ_big_int (Big_int_Z.succ_big_int (Big_int_Z.succ_big_int
-    (Big_int_Z.succ_big_int (Big_int_Z.succ_big_int (Big_int_Z.succ_big_int
-    (Big_int_Z.succ_big_int (Big_int_Z.succ_big_int (Big_int_Z.succ_big_int
-    (Big_int_Z.succ_big_int Big_int_Z.zero_big_int)))))))))
 
 (** val eRR_NONCANONICAL_LINE : Big_int_Z.big_int **)
 
@@ -470,6 +445,16 @@ let eRR_UNKNOWN_RULE =
     (Big_int_Z.succ_big_int (Big_int_Z.succ_big_int (Big_int_Z.succ_big_int
     (Big_int_Z.succ_big_int (Big_int_Z.succ_big_int (Big_int_Z.succ_big_int
     (Big_int_Z.succ_big_int Big_int_Z.zero_big_int))))))))))))
+
+(** val eRR_NORMALIZED_STEP_REJECTED : Big_int_Z.big_int **)
+
+let eRR_NORMALIZED_STEP_REJECTED =
+  Big_int_Z.succ_big_int (Big_int_Z.succ_big_int (Big_int_Z.succ_big_int
+    (Big_int_Z.succ_big_int (Big_int_Z.succ_big_int (Big_int_Z.succ_big_int
+    (Big_int_Z.succ_big_int (Big_int_Z.succ_big_int (Big_int_Z.succ_big_int
+    (Big_int_Z.succ_big_int (Big_int_Z.succ_big_int (Big_int_Z.succ_big_int
+    (Big_int_Z.succ_big_int (Big_int_Z.succ_big_int
+    Big_int_Z.zero_big_int)))))))))))))
 
 (** val eRR_NONCANONICAL_FORMULA : Big_int_Z.big_int **)
 
@@ -494,781 +479,6 @@ let eRR_BAD_FORMULA_TAG =
     (Big_int_Z.succ_big_int (Big_int_Z.succ_big_int (Big_int_Z.succ_big_int
     (Big_int_Z.succ_big_int (Big_int_Z.succ_big_int (Big_int_Z.succ_big_int
     Big_int_Z.zero_big_int))))))))))))))))))))
-
-(** val eRR_BAD_IMP_PAYLOAD : Big_int_Z.big_int **)
-
-let eRR_BAD_IMP_PAYLOAD =
-  Big_int_Z.succ_big_int (Big_int_Z.succ_big_int (Big_int_Z.succ_big_int
-    (Big_int_Z.succ_big_int (Big_int_Z.succ_big_int (Big_int_Z.succ_big_int
-    (Big_int_Z.succ_big_int (Big_int_Z.succ_big_int (Big_int_Z.succ_big_int
-    (Big_int_Z.succ_big_int (Big_int_Z.succ_big_int (Big_int_Z.succ_big_int
-    (Big_int_Z.succ_big_int (Big_int_Z.succ_big_int (Big_int_Z.succ_big_int
-    (Big_int_Z.succ_big_int (Big_int_Z.succ_big_int (Big_int_Z.succ_big_int
-    (Big_int_Z.succ_big_int (Big_int_Z.succ_big_int (Big_int_Z.succ_big_int
-    (Big_int_Z.succ_big_int (Big_int_Z.succ_big_int
-    Big_int_Z.zero_big_int))))))))))))))))))))))
-
-(** val eRR_NOT_IMP : Big_int_Z.big_int **)
-
-let eRR_NOT_IMP =
-  Big_int_Z.succ_big_int (Big_int_Z.succ_big_int (Big_int_Z.succ_big_int
-    (Big_int_Z.succ_big_int (Big_int_Z.succ_big_int (Big_int_Z.succ_big_int
-    (Big_int_Z.succ_big_int (Big_int_Z.succ_big_int (Big_int_Z.succ_big_int
-    (Big_int_Z.succ_big_int (Big_int_Z.succ_big_int (Big_int_Z.succ_big_int
-    (Big_int_Z.succ_big_int (Big_int_Z.succ_big_int (Big_int_Z.succ_big_int
-    (Big_int_Z.succ_big_int (Big_int_Z.succ_big_int (Big_int_Z.succ_big_int
-    (Big_int_Z.succ_big_int (Big_int_Z.succ_big_int (Big_int_Z.succ_big_int
-    (Big_int_Z.succ_big_int (Big_int_Z.succ_big_int (Big_int_Z.succ_big_int
-    Big_int_Z.zero_big_int)))))))))))))))))))))))
-
-(** val eRR_AXK_NOT_IMP_1 : Big_int_Z.big_int **)
-
-let eRR_AXK_NOT_IMP_1 =
-  Big_int_Z.succ_big_int (Big_int_Z.succ_big_int (Big_int_Z.succ_big_int
-    (Big_int_Z.succ_big_int (Big_int_Z.succ_big_int (Big_int_Z.succ_big_int
-    (Big_int_Z.succ_big_int (Big_int_Z.succ_big_int (Big_int_Z.succ_big_int
-    (Big_int_Z.succ_big_int (Big_int_Z.succ_big_int (Big_int_Z.succ_big_int
-    (Big_int_Z.succ_big_int (Big_int_Z.succ_big_int (Big_int_Z.succ_big_int
-    (Big_int_Z.succ_big_int (Big_int_Z.succ_big_int (Big_int_Z.succ_big_int
-    (Big_int_Z.succ_big_int (Big_int_Z.succ_big_int (Big_int_Z.succ_big_int
-    (Big_int_Z.succ_big_int (Big_int_Z.succ_big_int (Big_int_Z.succ_big_int
-    (Big_int_Z.succ_big_int (Big_int_Z.succ_big_int (Big_int_Z.succ_big_int
-    (Big_int_Z.succ_big_int (Big_int_Z.succ_big_int (Big_int_Z.succ_big_int
-    (Big_int_Z.succ_big_int (Big_int_Z.succ_big_int (Big_int_Z.succ_big_int
-    (Big_int_Z.succ_big_int (Big_int_Z.succ_big_int (Big_int_Z.succ_big_int
-    (Big_int_Z.succ_big_int (Big_int_Z.succ_big_int (Big_int_Z.succ_big_int
-    (Big_int_Z.succ_big_int
-    Big_int_Z.zero_big_int)))))))))))))))))))))))))))))))))))))))
-
-(** val eRR_AXK_NOT_IMP_2 : Big_int_Z.big_int **)
-
-let eRR_AXK_NOT_IMP_2 =
-  Big_int_Z.succ_big_int (Big_int_Z.succ_big_int (Big_int_Z.succ_big_int
-    (Big_int_Z.succ_big_int (Big_int_Z.succ_big_int (Big_int_Z.succ_big_int
-    (Big_int_Z.succ_big_int (Big_int_Z.succ_big_int (Big_int_Z.succ_big_int
-    (Big_int_Z.succ_big_int (Big_int_Z.succ_big_int (Big_int_Z.succ_big_int
-    (Big_int_Z.succ_big_int (Big_int_Z.succ_big_int (Big_int_Z.succ_big_int
-    (Big_int_Z.succ_big_int (Big_int_Z.succ_big_int (Big_int_Z.succ_big_int
-    (Big_int_Z.succ_big_int (Big_int_Z.succ_big_int (Big_int_Z.succ_big_int
-    (Big_int_Z.succ_big_int (Big_int_Z.succ_big_int (Big_int_Z.succ_big_int
-    (Big_int_Z.succ_big_int (Big_int_Z.succ_big_int (Big_int_Z.succ_big_int
-    (Big_int_Z.succ_big_int (Big_int_Z.succ_big_int (Big_int_Z.succ_big_int
-    (Big_int_Z.succ_big_int (Big_int_Z.succ_big_int (Big_int_Z.succ_big_int
-    (Big_int_Z.succ_big_int (Big_int_Z.succ_big_int (Big_int_Z.succ_big_int
-    (Big_int_Z.succ_big_int (Big_int_Z.succ_big_int (Big_int_Z.succ_big_int
-    (Big_int_Z.succ_big_int (Big_int_Z.succ_big_int
-    Big_int_Z.zero_big_int))))))))))))))))))))))))))))))))))))))))
-
-(** val eRR_AXK_A_MISMATCH : Big_int_Z.big_int **)
-
-let eRR_AXK_A_MISMATCH =
-  Big_int_Z.succ_big_int (Big_int_Z.succ_big_int (Big_int_Z.succ_big_int
-    (Big_int_Z.succ_big_int (Big_int_Z.succ_big_int (Big_int_Z.succ_big_int
-    (Big_int_Z.succ_big_int (Big_int_Z.succ_big_int (Big_int_Z.succ_big_int
-    (Big_int_Z.succ_big_int (Big_int_Z.succ_big_int (Big_int_Z.succ_big_int
-    (Big_int_Z.succ_big_int (Big_int_Z.succ_big_int (Big_int_Z.succ_big_int
-    (Big_int_Z.succ_big_int (Big_int_Z.succ_big_int (Big_int_Z.succ_big_int
-    (Big_int_Z.succ_big_int (Big_int_Z.succ_big_int (Big_int_Z.succ_big_int
-    (Big_int_Z.succ_big_int (Big_int_Z.succ_big_int (Big_int_Z.succ_big_int
-    (Big_int_Z.succ_big_int (Big_int_Z.succ_big_int (Big_int_Z.succ_big_int
-    (Big_int_Z.succ_big_int (Big_int_Z.succ_big_int (Big_int_Z.succ_big_int
-    (Big_int_Z.succ_big_int (Big_int_Z.succ_big_int (Big_int_Z.succ_big_int
-    (Big_int_Z.succ_big_int (Big_int_Z.succ_big_int (Big_int_Z.succ_big_int
-    (Big_int_Z.succ_big_int (Big_int_Z.succ_big_int (Big_int_Z.succ_big_int
-    (Big_int_Z.succ_big_int (Big_int_Z.succ_big_int (Big_int_Z.succ_big_int
-    Big_int_Z.zero_big_int)))))))))))))))))))))))))))))))))))))))))
-
-(** val eRR_AXK_BAD_A : Big_int_Z.big_int **)
-
-let eRR_AXK_BAD_A =
-  Big_int_Z.succ_big_int (Big_int_Z.succ_big_int (Big_int_Z.succ_big_int
-    (Big_int_Z.succ_big_int (Big_int_Z.succ_big_int (Big_int_Z.succ_big_int
-    (Big_int_Z.succ_big_int (Big_int_Z.succ_big_int (Big_int_Z.succ_big_int
-    (Big_int_Z.succ_big_int (Big_int_Z.succ_big_int (Big_int_Z.succ_big_int
-    (Big_int_Z.succ_big_int (Big_int_Z.succ_big_int (Big_int_Z.succ_big_int
-    (Big_int_Z.succ_big_int (Big_int_Z.succ_big_int (Big_int_Z.succ_big_int
-    (Big_int_Z.succ_big_int (Big_int_Z.succ_big_int (Big_int_Z.succ_big_int
-    (Big_int_Z.succ_big_int (Big_int_Z.succ_big_int (Big_int_Z.succ_big_int
-    (Big_int_Z.succ_big_int (Big_int_Z.succ_big_int (Big_int_Z.succ_big_int
-    (Big_int_Z.succ_big_int (Big_int_Z.succ_big_int (Big_int_Z.succ_big_int
-    (Big_int_Z.succ_big_int (Big_int_Z.succ_big_int (Big_int_Z.succ_big_int
-    (Big_int_Z.succ_big_int (Big_int_Z.succ_big_int (Big_int_Z.succ_big_int
-    (Big_int_Z.succ_big_int (Big_int_Z.succ_big_int (Big_int_Z.succ_big_int
-    (Big_int_Z.succ_big_int (Big_int_Z.succ_big_int (Big_int_Z.succ_big_int
-    (Big_int_Z.succ_big_int
-    Big_int_Z.zero_big_int))))))))))))))))))))))))))))))))))))))))))
-
-(** val eRR_AXK_BAD_B : Big_int_Z.big_int **)
-
-let eRR_AXK_BAD_B =
-  Big_int_Z.succ_big_int (Big_int_Z.succ_big_int (Big_int_Z.succ_big_int
-    (Big_int_Z.succ_big_int (Big_int_Z.succ_big_int (Big_int_Z.succ_big_int
-    (Big_int_Z.succ_big_int (Big_int_Z.succ_big_int (Big_int_Z.succ_big_int
-    (Big_int_Z.succ_big_int (Big_int_Z.succ_big_int (Big_int_Z.succ_big_int
-    (Big_int_Z.succ_big_int (Big_int_Z.succ_big_int (Big_int_Z.succ_big_int
-    (Big_int_Z.succ_big_int (Big_int_Z.succ_big_int (Big_int_Z.succ_big_int
-    (Big_int_Z.succ_big_int (Big_int_Z.succ_big_int (Big_int_Z.succ_big_int
-    (Big_int_Z.succ_big_int (Big_int_Z.succ_big_int (Big_int_Z.succ_big_int
-    (Big_int_Z.succ_big_int (Big_int_Z.succ_big_int (Big_int_Z.succ_big_int
-    (Big_int_Z.succ_big_int (Big_int_Z.succ_big_int (Big_int_Z.succ_big_int
-    (Big_int_Z.succ_big_int (Big_int_Z.succ_big_int (Big_int_Z.succ_big_int
-    (Big_int_Z.succ_big_int (Big_int_Z.succ_big_int (Big_int_Z.succ_big_int
-    (Big_int_Z.succ_big_int (Big_int_Z.succ_big_int (Big_int_Z.succ_big_int
-    (Big_int_Z.succ_big_int (Big_int_Z.succ_big_int (Big_int_Z.succ_big_int
-    (Big_int_Z.succ_big_int (Big_int_Z.succ_big_int
-    Big_int_Z.zero_big_int)))))))))))))))))))))))))))))))))))))))))))
-
-(** val eRR_AXS_NOT_IMP_1 : Big_int_Z.big_int **)
-
-let eRR_AXS_NOT_IMP_1 =
-  Big_int_Z.succ_big_int (Big_int_Z.succ_big_int (Big_int_Z.succ_big_int
-    (Big_int_Z.succ_big_int (Big_int_Z.succ_big_int (Big_int_Z.succ_big_int
-    (Big_int_Z.succ_big_int (Big_int_Z.succ_big_int (Big_int_Z.succ_big_int
-    (Big_int_Z.succ_big_int (Big_int_Z.succ_big_int (Big_int_Z.succ_big_int
-    (Big_int_Z.succ_big_int (Big_int_Z.succ_big_int (Big_int_Z.succ_big_int
-    (Big_int_Z.succ_big_int (Big_int_Z.succ_big_int (Big_int_Z.succ_big_int
-    (Big_int_Z.succ_big_int (Big_int_Z.succ_big_int (Big_int_Z.succ_big_int
-    (Big_int_Z.succ_big_int (Big_int_Z.succ_big_int (Big_int_Z.succ_big_int
-    (Big_int_Z.succ_big_int (Big_int_Z.succ_big_int (Big_int_Z.succ_big_int
-    (Big_int_Z.succ_big_int (Big_int_Z.succ_big_int (Big_int_Z.succ_big_int
-    (Big_int_Z.succ_big_int (Big_int_Z.succ_big_int (Big_int_Z.succ_big_int
-    (Big_int_Z.succ_big_int (Big_int_Z.succ_big_int (Big_int_Z.succ_big_int
-    (Big_int_Z.succ_big_int (Big_int_Z.succ_big_int (Big_int_Z.succ_big_int
-    (Big_int_Z.succ_big_int (Big_int_Z.succ_big_int (Big_int_Z.succ_big_int
-    (Big_int_Z.succ_big_int (Big_int_Z.succ_big_int (Big_int_Z.succ_big_int
-    (Big_int_Z.succ_big_int (Big_int_Z.succ_big_int (Big_int_Z.succ_big_int
-    (Big_int_Z.succ_big_int (Big_int_Z.succ_big_int (Big_int_Z.succ_big_int
-    (Big_int_Z.succ_big_int (Big_int_Z.succ_big_int (Big_int_Z.succ_big_int
-    (Big_int_Z.succ_big_int (Big_int_Z.succ_big_int (Big_int_Z.succ_big_int
-    (Big_int_Z.succ_big_int (Big_int_Z.succ_big_int (Big_int_Z.succ_big_int
-    Big_int_Z.zero_big_int)))))))))))))))))))))))))))))))))))))))))))))))))))))))))))
-
-(** val eRR_AXS_NOT_IMP_2 : Big_int_Z.big_int **)
-
-let eRR_AXS_NOT_IMP_2 =
-  Big_int_Z.succ_big_int (Big_int_Z.succ_big_int (Big_int_Z.succ_big_int
-    (Big_int_Z.succ_big_int (Big_int_Z.succ_big_int (Big_int_Z.succ_big_int
-    (Big_int_Z.succ_big_int (Big_int_Z.succ_big_int (Big_int_Z.succ_big_int
-    (Big_int_Z.succ_big_int (Big_int_Z.succ_big_int (Big_int_Z.succ_big_int
-    (Big_int_Z.succ_big_int (Big_int_Z.succ_big_int (Big_int_Z.succ_big_int
-    (Big_int_Z.succ_big_int (Big_int_Z.succ_big_int (Big_int_Z.succ_big_int
-    (Big_int_Z.succ_big_int (Big_int_Z.succ_big_int (Big_int_Z.succ_big_int
-    (Big_int_Z.succ_big_int (Big_int_Z.succ_big_int (Big_int_Z.succ_big_int
-    (Big_int_Z.succ_big_int (Big_int_Z.succ_big_int (Big_int_Z.succ_big_int
-    (Big_int_Z.succ_big_int (Big_int_Z.succ_big_int (Big_int_Z.succ_big_int
-    (Big_int_Z.succ_big_int (Big_int_Z.succ_big_int (Big_int_Z.succ_big_int
-    (Big_int_Z.succ_big_int (Big_int_Z.succ_big_int (Big_int_Z.succ_big_int
-    (Big_int_Z.succ_big_int (Big_int_Z.succ_big_int (Big_int_Z.succ_big_int
-    (Big_int_Z.succ_big_int (Big_int_Z.succ_big_int (Big_int_Z.succ_big_int
-    (Big_int_Z.succ_big_int (Big_int_Z.succ_big_int (Big_int_Z.succ_big_int
-    (Big_int_Z.succ_big_int (Big_int_Z.succ_big_int (Big_int_Z.succ_big_int
-    (Big_int_Z.succ_big_int (Big_int_Z.succ_big_int (Big_int_Z.succ_big_int
-    (Big_int_Z.succ_big_int (Big_int_Z.succ_big_int (Big_int_Z.succ_big_int
-    (Big_int_Z.succ_big_int (Big_int_Z.succ_big_int (Big_int_Z.succ_big_int
-    (Big_int_Z.succ_big_int (Big_int_Z.succ_big_int (Big_int_Z.succ_big_int
-    (Big_int_Z.succ_big_int
-    Big_int_Z.zero_big_int))))))))))))))))))))))))))))))))))))))))))))))))))))))))))))
-
-(** val eRR_AXS_NOT_IMP_3 : Big_int_Z.big_int **)
-
-let eRR_AXS_NOT_IMP_3 =
-  Big_int_Z.succ_big_int (Big_int_Z.succ_big_int (Big_int_Z.succ_big_int
-    (Big_int_Z.succ_big_int (Big_int_Z.succ_big_int (Big_int_Z.succ_big_int
-    (Big_int_Z.succ_big_int (Big_int_Z.succ_big_int (Big_int_Z.succ_big_int
-    (Big_int_Z.succ_big_int (Big_int_Z.succ_big_int (Big_int_Z.succ_big_int
-    (Big_int_Z.succ_big_int (Big_int_Z.succ_big_int (Big_int_Z.succ_big_int
-    (Big_int_Z.succ_big_int (Big_int_Z.succ_big_int (Big_int_Z.succ_big_int
-    (Big_int_Z.succ_big_int (Big_int_Z.succ_big_int (Big_int_Z.succ_big_int
-    (Big_int_Z.succ_big_int (Big_int_Z.succ_big_int (Big_int_Z.succ_big_int
-    (Big_int_Z.succ_big_int (Big_int_Z.succ_big_int (Big_int_Z.succ_big_int
-    (Big_int_Z.succ_big_int (Big_int_Z.succ_big_int (Big_int_Z.succ_big_int
-    (Big_int_Z.succ_big_int (Big_int_Z.succ_big_int (Big_int_Z.succ_big_int
-    (Big_int_Z.succ_big_int (Big_int_Z.succ_big_int (Big_int_Z.succ_big_int
-    (Big_int_Z.succ_big_int (Big_int_Z.succ_big_int (Big_int_Z.succ_big_int
-    (Big_int_Z.succ_big_int (Big_int_Z.succ_big_int (Big_int_Z.succ_big_int
-    (Big_int_Z.succ_big_int (Big_int_Z.succ_big_int (Big_int_Z.succ_big_int
-    (Big_int_Z.succ_big_int (Big_int_Z.succ_big_int (Big_int_Z.succ_big_int
-    (Big_int_Z.succ_big_int (Big_int_Z.succ_big_int (Big_int_Z.succ_big_int
-    (Big_int_Z.succ_big_int (Big_int_Z.succ_big_int (Big_int_Z.succ_big_int
-    (Big_int_Z.succ_big_int (Big_int_Z.succ_big_int (Big_int_Z.succ_big_int
-    (Big_int_Z.succ_big_int (Big_int_Z.succ_big_int (Big_int_Z.succ_big_int
-    (Big_int_Z.succ_big_int (Big_int_Z.succ_big_int
-    Big_int_Z.zero_big_int)))))))))))))))))))))))))))))))))))))))))))))))))))))))))))))
-
-(** val eRR_AXS_NOT_IMP_4 : Big_int_Z.big_int **)
-
-let eRR_AXS_NOT_IMP_4 =
-  Big_int_Z.succ_big_int (Big_int_Z.succ_big_int (Big_int_Z.succ_big_int
-    (Big_int_Z.succ_big_int (Big_int_Z.succ_big_int (Big_int_Z.succ_big_int
-    (Big_int_Z.succ_big_int (Big_int_Z.succ_big_int (Big_int_Z.succ_big_int
-    (Big_int_Z.succ_big_int (Big_int_Z.succ_big_int (Big_int_Z.succ_big_int
-    (Big_int_Z.succ_big_int (Big_int_Z.succ_big_int (Big_int_Z.succ_big_int
-    (Big_int_Z.succ_big_int (Big_int_Z.succ_big_int (Big_int_Z.succ_big_int
-    (Big_int_Z.succ_big_int (Big_int_Z.succ_big_int (Big_int_Z.succ_big_int
-    (Big_int_Z.succ_big_int (Big_int_Z.succ_big_int (Big_int_Z.succ_big_int
-    (Big_int_Z.succ_big_int (Big_int_Z.succ_big_int (Big_int_Z.succ_big_int
-    (Big_int_Z.succ_big_int (Big_int_Z.succ_big_int (Big_int_Z.succ_big_int
-    (Big_int_Z.succ_big_int (Big_int_Z.succ_big_int (Big_int_Z.succ_big_int
-    (Big_int_Z.succ_big_int (Big_int_Z.succ_big_int (Big_int_Z.succ_big_int
-    (Big_int_Z.succ_big_int (Big_int_Z.succ_big_int (Big_int_Z.succ_big_int
-    (Big_int_Z.succ_big_int (Big_int_Z.succ_big_int (Big_int_Z.succ_big_int
-    (Big_int_Z.succ_big_int (Big_int_Z.succ_big_int (Big_int_Z.succ_big_int
-    (Big_int_Z.succ_big_int (Big_int_Z.succ_big_int (Big_int_Z.succ_big_int
-    (Big_int_Z.succ_big_int (Big_int_Z.succ_big_int (Big_int_Z.succ_big_int
-    (Big_int_Z.succ_big_int (Big_int_Z.succ_big_int (Big_int_Z.succ_big_int
-    (Big_int_Z.succ_big_int (Big_int_Z.succ_big_int (Big_int_Z.succ_big_int
-    (Big_int_Z.succ_big_int (Big_int_Z.succ_big_int (Big_int_Z.succ_big_int
-    (Big_int_Z.succ_big_int (Big_int_Z.succ_big_int (Big_int_Z.succ_big_int
-    Big_int_Z.zero_big_int))))))))))))))))))))))))))))))))))))))))))))))))))))))))))))))
-
-(** val eRR_AXS_NOT_IMP_5 : Big_int_Z.big_int **)
-
-let eRR_AXS_NOT_IMP_5 =
-  Big_int_Z.succ_big_int (Big_int_Z.succ_big_int (Big_int_Z.succ_big_int
-    (Big_int_Z.succ_big_int (Big_int_Z.succ_big_int (Big_int_Z.succ_big_int
-    (Big_int_Z.succ_big_int (Big_int_Z.succ_big_int (Big_int_Z.succ_big_int
-    (Big_int_Z.succ_big_int (Big_int_Z.succ_big_int (Big_int_Z.succ_big_int
-    (Big_int_Z.succ_big_int (Big_int_Z.succ_big_int (Big_int_Z.succ_big_int
-    (Big_int_Z.succ_big_int (Big_int_Z.succ_big_int (Big_int_Z.succ_big_int
-    (Big_int_Z.succ_big_int (Big_int_Z.succ_big_int (Big_int_Z.succ_big_int
-    (Big_int_Z.succ_big_int (Big_int_Z.succ_big_int (Big_int_Z.succ_big_int
-    (Big_int_Z.succ_big_int (Big_int_Z.succ_big_int (Big_int_Z.succ_big_int
-    (Big_int_Z.succ_big_int (Big_int_Z.succ_big_int (Big_int_Z.succ_big_int
-    (Big_int_Z.succ_big_int (Big_int_Z.succ_big_int (Big_int_Z.succ_big_int
-    (Big_int_Z.succ_big_int (Big_int_Z.succ_big_int (Big_int_Z.succ_big_int
-    (Big_int_Z.succ_big_int (Big_int_Z.succ_big_int (Big_int_Z.succ_big_int
-    (Big_int_Z.succ_big_int (Big_int_Z.succ_big_int (Big_int_Z.succ_big_int
-    (Big_int_Z.succ_big_int (Big_int_Z.succ_big_int (Big_int_Z.succ_big_int
-    (Big_int_Z.succ_big_int (Big_int_Z.succ_big_int (Big_int_Z.succ_big_int
-    (Big_int_Z.succ_big_int (Big_int_Z.succ_big_int (Big_int_Z.succ_big_int
-    (Big_int_Z.succ_big_int (Big_int_Z.succ_big_int (Big_int_Z.succ_big_int
-    (Big_int_Z.succ_big_int (Big_int_Z.succ_big_int (Big_int_Z.succ_big_int
-    (Big_int_Z.succ_big_int (Big_int_Z.succ_big_int (Big_int_Z.succ_big_int
-    (Big_int_Z.succ_big_int (Big_int_Z.succ_big_int (Big_int_Z.succ_big_int
-    (Big_int_Z.succ_big_int
-    Big_int_Z.zero_big_int)))))))))))))))))))))))))))))))))))))))))))))))))))))))))))))))
-
-(** val eRR_AXS_NOT_IMP_6 : Big_int_Z.big_int **)
-
-let eRR_AXS_NOT_IMP_6 =
-  Big_int_Z.succ_big_int (Big_int_Z.succ_big_int (Big_int_Z.succ_big_int
-    (Big_int_Z.succ_big_int (Big_int_Z.succ_big_int (Big_int_Z.succ_big_int
-    (Big_int_Z.succ_big_int (Big_int_Z.succ_big_int (Big_int_Z.succ_big_int
-    (Big_int_Z.succ_big_int (Big_int_Z.succ_big_int (Big_int_Z.succ_big_int
-    (Big_int_Z.succ_big_int (Big_int_Z.succ_big_int (Big_int_Z.succ_big_int
-    (Big_int_Z.succ_big_int (Big_int_Z.succ_big_int (Big_int_Z.succ_big_int
-    (Big_int_Z.succ_big_int (Big_int_Z.succ_big_int (Big_int_Z.succ_big_int
-    (Big_int_Z.succ_big_int (Big_int_Z.succ_big_int (Big_int_Z.succ_big_int
-    (Big_int_Z.succ_big_int (Big_int_Z.succ_big_int (Big_int_Z.succ_big_int
-    (Big_int_Z.succ_big_int (Big_int_Z.succ_big_int (Big_int_Z.succ_big_int
-    (Big_int_Z.succ_big_int (Big_int_Z.succ_big_int (Big_int_Z.succ_big_int
-    (Big_int_Z.succ_big_int (Big_int_Z.succ_big_int (Big_int_Z.succ_big_int
-    (Big_int_Z.succ_big_int (Big_int_Z.succ_big_int (Big_int_Z.succ_big_int
-    (Big_int_Z.succ_big_int (Big_int_Z.succ_big_int (Big_int_Z.succ_big_int
-    (Big_int_Z.succ_big_int (Big_int_Z.succ_big_int (Big_int_Z.succ_big_int
-    (Big_int_Z.succ_big_int (Big_int_Z.succ_big_int (Big_int_Z.succ_big_int
-    (Big_int_Z.succ_big_int (Big_int_Z.succ_big_int (Big_int_Z.succ_big_int
-    (Big_int_Z.succ_big_int (Big_int_Z.succ_big_int (Big_int_Z.succ_big_int
-    (Big_int_Z.succ_big_int (Big_int_Z.succ_big_int (Big_int_Z.succ_big_int
-    (Big_int_Z.succ_big_int (Big_int_Z.succ_big_int (Big_int_Z.succ_big_int
-    (Big_int_Z.succ_big_int (Big_int_Z.succ_big_int (Big_int_Z.succ_big_int
-    (Big_int_Z.succ_big_int (Big_int_Z.succ_big_int
-    Big_int_Z.zero_big_int))))))))))))))))))))))))))))))))))))))))))))))))))))))))))))))))
-
-(** val eRR_AXS_A_MISMATCH_LEFT : Big_int_Z.big_int **)
-
-let eRR_AXS_A_MISMATCH_LEFT =
-  Big_int_Z.succ_big_int (Big_int_Z.succ_big_int (Big_int_Z.succ_big_int
-    (Big_int_Z.succ_big_int (Big_int_Z.succ_big_int (Big_int_Z.succ_big_int
-    (Big_int_Z.succ_big_int (Big_int_Z.succ_big_int (Big_int_Z.succ_big_int
-    (Big_int_Z.succ_big_int (Big_int_Z.succ_big_int (Big_int_Z.succ_big_int
-    (Big_int_Z.succ_big_int (Big_int_Z.succ_big_int (Big_int_Z.succ_big_int
-    (Big_int_Z.succ_big_int (Big_int_Z.succ_big_int (Big_int_Z.succ_big_int
-    (Big_int_Z.succ_big_int (Big_int_Z.succ_big_int (Big_int_Z.succ_big_int
-    (Big_int_Z.succ_big_int (Big_int_Z.succ_big_int (Big_int_Z.succ_big_int
-    (Big_int_Z.succ_big_int (Big_int_Z.succ_big_int (Big_int_Z.succ_big_int
-    (Big_int_Z.succ_big_int (Big_int_Z.succ_big_int (Big_int_Z.succ_big_int
-    (Big_int_Z.succ_big_int (Big_int_Z.succ_big_int (Big_int_Z.succ_big_int
-    (Big_int_Z.succ_big_int (Big_int_Z.succ_big_int (Big_int_Z.succ_big_int
-    (Big_int_Z.succ_big_int (Big_int_Z.succ_big_int (Big_int_Z.succ_big_int
-    (Big_int_Z.succ_big_int (Big_int_Z.succ_big_int (Big_int_Z.succ_big_int
-    (Big_int_Z.succ_big_int (Big_int_Z.succ_big_int (Big_int_Z.succ_big_int
-    (Big_int_Z.succ_big_int (Big_int_Z.succ_big_int (Big_int_Z.succ_big_int
-    (Big_int_Z.succ_big_int (Big_int_Z.succ_big_int (Big_int_Z.succ_big_int
-    (Big_int_Z.succ_big_int (Big_int_Z.succ_big_int (Big_int_Z.succ_big_int
-    (Big_int_Z.succ_big_int (Big_int_Z.succ_big_int (Big_int_Z.succ_big_int
-    (Big_int_Z.succ_big_int (Big_int_Z.succ_big_int (Big_int_Z.succ_big_int
-    (Big_int_Z.succ_big_int (Big_int_Z.succ_big_int (Big_int_Z.succ_big_int
-    (Big_int_Z.succ_big_int (Big_int_Z.succ_big_int (Big_int_Z.succ_big_int
-    Big_int_Z.zero_big_int)))))))))))))))))))))))))))))))))))))))))))))))))))))))))))))))))
-
-(** val eRR_AXS_A_MISMATCH_RIGHT : Big_int_Z.big_int **)
-
-let eRR_AXS_A_MISMATCH_RIGHT =
-  Big_int_Z.succ_big_int (Big_int_Z.succ_big_int (Big_int_Z.succ_big_int
-    (Big_int_Z.succ_big_int (Big_int_Z.succ_big_int (Big_int_Z.succ_big_int
-    (Big_int_Z.succ_big_int (Big_int_Z.succ_big_int (Big_int_Z.succ_big_int
-    (Big_int_Z.succ_big_int (Big_int_Z.succ_big_int (Big_int_Z.succ_big_int
-    (Big_int_Z.succ_big_int (Big_int_Z.succ_big_int (Big_int_Z.succ_big_int
-    (Big_int_Z.succ_big_int (Big_int_Z.succ_big_int (Big_int_Z.succ_big_int
-    (Big_int_Z.succ_big_int (Big_int_Z.succ_big_int (Big_int_Z.succ_big_int
-    (Big_int_Z.succ_big_int (Big_int_Z.succ_big_int (Big_int_Z.succ_big_int
-    (Big_int_Z.succ_big_int (Big_int_Z.succ_big_int (Big_int_Z.succ_big_int
-    (Big_int_Z.succ_big_int (Big_int_Z.succ_big_int (Big_int_Z.succ_big_int
-    (Big_int_Z.succ_big_int (Big_int_Z.succ_big_int (Big_int_Z.succ_big_int
-    (Big_int_Z.succ_big_int (Big_int_Z.succ_big_int (Big_int_Z.succ_big_int
-    (Big_int_Z.succ_big_int (Big_int_Z.succ_big_int (Big_int_Z.succ_big_int
-    (Big_int_Z.succ_big_int (Big_int_Z.succ_big_int (Big_int_Z.succ_big_int
-    (Big_int_Z.succ_big_int (Big_int_Z.succ_big_int (Big_int_Z.succ_big_int
-    (Big_int_Z.succ_big_int (Big_int_Z.succ_big_int (Big_int_Z.succ_big_int
-    (Big_int_Z.succ_big_int (Big_int_Z.succ_big_int (Big_int_Z.succ_big_int
-    (Big_int_Z.succ_big_int (Big_int_Z.succ_big_int (Big_int_Z.succ_big_int
-    (Big_int_Z.succ_big_int (Big_int_Z.succ_big_int (Big_int_Z.succ_big_int
-    (Big_int_Z.succ_big_int (Big_int_Z.succ_big_int (Big_int_Z.succ_big_int
-    (Big_int_Z.succ_big_int (Big_int_Z.succ_big_int (Big_int_Z.succ_big_int
-    (Big_int_Z.succ_big_int (Big_int_Z.succ_big_int (Big_int_Z.succ_big_int
-    (Big_int_Z.succ_big_int
-    Big_int_Z.zero_big_int))))))))))))))))))))))))))))))))))))))))))))))))))))))))))))))))))
-
-(** val eRR_AXS_B_MISMATCH : Big_int_Z.big_int **)
-
-let eRR_AXS_B_MISMATCH =
-  Big_int_Z.succ_big_int (Big_int_Z.succ_big_int (Big_int_Z.succ_big_int
-    (Big_int_Z.succ_big_int (Big_int_Z.succ_big_int (Big_int_Z.succ_big_int
-    (Big_int_Z.succ_big_int (Big_int_Z.succ_big_int (Big_int_Z.succ_big_int
-    (Big_int_Z.succ_big_int (Big_int_Z.succ_big_int (Big_int_Z.succ_big_int
-    (Big_int_Z.succ_big_int (Big_int_Z.succ_big_int (Big_int_Z.succ_big_int
-    (Big_int_Z.succ_big_int (Big_int_Z.succ_big_int (Big_int_Z.succ_big_int
-    (Big_int_Z.succ_big_int (Big_int_Z.succ_big_int (Big_int_Z.succ_big_int
-    (Big_int_Z.succ_big_int (Big_int_Z.succ_big_int (Big_int_Z.succ_big_int
-    (Big_int_Z.succ_big_int (Big_int_Z.succ_big_int (Big_int_Z.succ_big_int
-    (Big_int_Z.succ_big_int (Big_int_Z.succ_big_int (Big_int_Z.succ_big_int
-    (Big_int_Z.succ_big_int (Big_int_Z.succ_big_int (Big_int_Z.succ_big_int
-    (Big_int_Z.succ_big_int (Big_int_Z.succ_big_int (Big_int_Z.succ_big_int
-    (Big_int_Z.succ_big_int (Big_int_Z.succ_big_int (Big_int_Z.succ_big_int
-    (Big_int_Z.succ_big_int (Big_int_Z.succ_big_int (Big_int_Z.succ_big_int
-    (Big_int_Z.succ_big_int (Big_int_Z.succ_big_int (Big_int_Z.succ_big_int
-    (Big_int_Z.succ_big_int (Big_int_Z.succ_big_int (Big_int_Z.succ_big_int
-    (Big_int_Z.succ_big_int (Big_int_Z.succ_big_int (Big_int_Z.succ_big_int
-    (Big_int_Z.succ_big_int (Big_int_Z.succ_big_int (Big_int_Z.succ_big_int
-    (Big_int_Z.succ_big_int (Big_int_Z.succ_big_int (Big_int_Z.succ_big_int
-    (Big_int_Z.succ_big_int (Big_int_Z.succ_big_int (Big_int_Z.succ_big_int
-    (Big_int_Z.succ_big_int (Big_int_Z.succ_big_int (Big_int_Z.succ_big_int
-    (Big_int_Z.succ_big_int (Big_int_Z.succ_big_int (Big_int_Z.succ_big_int
-    (Big_int_Z.succ_big_int (Big_int_Z.succ_big_int
-    Big_int_Z.zero_big_int)))))))))))))))))))))))))))))))))))))))))))))))))))))))))))))))))))
-
-(** val eRR_AXS_C_MISMATCH : Big_int_Z.big_int **)
-
-let eRR_AXS_C_MISMATCH =
-  Big_int_Z.succ_big_int (Big_int_Z.succ_big_int (Big_int_Z.succ_big_int
-    (Big_int_Z.succ_big_int (Big_int_Z.succ_big_int (Big_int_Z.succ_big_int
-    (Big_int_Z.succ_big_int (Big_int_Z.succ_big_int (Big_int_Z.succ_big_int
-    (Big_int_Z.succ_big_int (Big_int_Z.succ_big_int (Big_int_Z.succ_big_int
-    (Big_int_Z.succ_big_int (Big_int_Z.succ_big_int (Big_int_Z.succ_big_int
-    (Big_int_Z.succ_big_int (Big_int_Z.succ_big_int (Big_int_Z.succ_big_int
-    (Big_int_Z.succ_big_int (Big_int_Z.succ_big_int (Big_int_Z.succ_big_int
-    (Big_int_Z.succ_big_int (Big_int_Z.succ_big_int (Big_int_Z.succ_big_int
-    (Big_int_Z.succ_big_int (Big_int_Z.succ_big_int (Big_int_Z.succ_big_int
-    (Big_int_Z.succ_big_int (Big_int_Z.succ_big_int (Big_int_Z.succ_big_int
-    (Big_int_Z.succ_big_int (Big_int_Z.succ_big_int (Big_int_Z.succ_big_int
-    (Big_int_Z.succ_big_int (Big_int_Z.succ_big_int (Big_int_Z.succ_big_int
-    (Big_int_Z.succ_big_int (Big_int_Z.succ_big_int (Big_int_Z.succ_big_int
-    (Big_int_Z.succ_big_int (Big_int_Z.succ_big_int (Big_int_Z.succ_big_int
-    (Big_int_Z.succ_big_int (Big_int_Z.succ_big_int (Big_int_Z.succ_big_int
-    (Big_int_Z.succ_big_int (Big_int_Z.succ_big_int (Big_int_Z.succ_big_int
-    (Big_int_Z.succ_big_int (Big_int_Z.succ_big_int (Big_int_Z.succ_big_int
-    (Big_int_Z.succ_big_int (Big_int_Z.succ_big_int (Big_int_Z.succ_big_int
-    (Big_int_Z.succ_big_int (Big_int_Z.succ_big_int (Big_int_Z.succ_big_int
-    (Big_int_Z.succ_big_int (Big_int_Z.succ_big_int (Big_int_Z.succ_big_int
-    (Big_int_Z.succ_big_int (Big_int_Z.succ_big_int (Big_int_Z.succ_big_int
-    (Big_int_Z.succ_big_int (Big_int_Z.succ_big_int (Big_int_Z.succ_big_int
-    (Big_int_Z.succ_big_int (Big_int_Z.succ_big_int (Big_int_Z.succ_big_int
-    Big_int_Z.zero_big_int))))))))))))))))))))))))))))))))))))))))))))))))))))))))))))))))))))
-
-(** val eRR_AXS_BAD_A : Big_int_Z.big_int **)
-
-let eRR_AXS_BAD_A =
-  Big_int_Z.succ_big_int (Big_int_Z.succ_big_int (Big_int_Z.succ_big_int
-    (Big_int_Z.succ_big_int (Big_int_Z.succ_big_int (Big_int_Z.succ_big_int
-    (Big_int_Z.succ_big_int (Big_int_Z.succ_big_int (Big_int_Z.succ_big_int
-    (Big_int_Z.succ_big_int (Big_int_Z.succ_big_int (Big_int_Z.succ_big_int
-    (Big_int_Z.succ_big_int (Big_int_Z.succ_big_int (Big_int_Z.succ_big_int
-    (Big_int_Z.succ_big_int (Big_int_Z.succ_big_int (Big_int_Z.succ_big_int
-    (Big_int_Z.succ_big_int (Big_int_Z.succ_big_int (Big_int_Z.succ_big_int
-    (Big_int_Z.succ_big_int (Big_int_Z.succ_big_int (Big_int_Z.succ_big_int
-    (Big_int_Z.succ_big_int (Big_int_Z.succ_big_int (Big_int_Z.succ_big_int
-    (Big_int_Z.succ_big_int (Big_int_Z.succ_big_int (Big_int_Z.succ_big_int
-    (Big_int_Z.succ_big_int (Big_int_Z.succ_big_int (Big_int_Z.succ_big_int
-    (Big_int_Z.succ_big_int (Big_int_Z.succ_big_int (Big_int_Z.succ_big_int
-    (Big_int_Z.succ_big_int (Big_int_Z.succ_big_int (Big_int_Z.succ_big_int
-    (Big_int_Z.succ_big_int (Big_int_Z.succ_big_int (Big_int_Z.succ_big_int
-    (Big_int_Z.succ_big_int (Big_int_Z.succ_big_int (Big_int_Z.succ_big_int
-    (Big_int_Z.succ_big_int (Big_int_Z.succ_big_int (Big_int_Z.succ_big_int
-    (Big_int_Z.succ_big_int (Big_int_Z.succ_big_int (Big_int_Z.succ_big_int
-    (Big_int_Z.succ_big_int (Big_int_Z.succ_big_int (Big_int_Z.succ_big_int
-    (Big_int_Z.succ_big_int (Big_int_Z.succ_big_int (Big_int_Z.succ_big_int
-    (Big_int_Z.succ_big_int (Big_int_Z.succ_big_int (Big_int_Z.succ_big_int
-    (Big_int_Z.succ_big_int (Big_int_Z.succ_big_int (Big_int_Z.succ_big_int
-    (Big_int_Z.succ_big_int (Big_int_Z.succ_big_int (Big_int_Z.succ_big_int
-    (Big_int_Z.succ_big_int (Big_int_Z.succ_big_int (Big_int_Z.succ_big_int
-    (Big_int_Z.succ_big_int
-    Big_int_Z.zero_big_int)))))))))))))))))))))))))))))))))))))))))))))))))))))))))))))))))))))
-
-(** val eRR_AXS_BAD_B : Big_int_Z.big_int **)
-
-let eRR_AXS_BAD_B =
-  Big_int_Z.succ_big_int (Big_int_Z.succ_big_int (Big_int_Z.succ_big_int
-    (Big_int_Z.succ_big_int (Big_int_Z.succ_big_int (Big_int_Z.succ_big_int
-    (Big_int_Z.succ_big_int (Big_int_Z.succ_big_int (Big_int_Z.succ_big_int
-    (Big_int_Z.succ_big_int (Big_int_Z.succ_big_int (Big_int_Z.succ_big_int
-    (Big_int_Z.succ_big_int (Big_int_Z.succ_big_int (Big_int_Z.succ_big_int
-    (Big_int_Z.succ_big_int (Big_int_Z.succ_big_int (Big_int_Z.succ_big_int
-    (Big_int_Z.succ_big_int (Big_int_Z.succ_big_int (Big_int_Z.succ_big_int
-    (Big_int_Z.succ_big_int (Big_int_Z.succ_big_int (Big_int_Z.succ_big_int
-    (Big_int_Z.succ_big_int (Big_int_Z.succ_big_int (Big_int_Z.succ_big_int
-    (Big_int_Z.succ_big_int (Big_int_Z.succ_big_int (Big_int_Z.succ_big_int
-    (Big_int_Z.succ_big_int (Big_int_Z.succ_big_int (Big_int_Z.succ_big_int
-    (Big_int_Z.succ_big_int (Big_int_Z.succ_big_int (Big_int_Z.succ_big_int
-    (Big_int_Z.succ_big_int (Big_int_Z.succ_big_int (Big_int_Z.succ_big_int
-    (Big_int_Z.succ_big_int (Big_int_Z.succ_big_int (Big_int_Z.succ_big_int
-    (Big_int_Z.succ_big_int (Big_int_Z.succ_big_int (Big_int_Z.succ_big_int
-    (Big_int_Z.succ_big_int (Big_int_Z.succ_big_int (Big_int_Z.succ_big_int
-    (Big_int_Z.succ_big_int (Big_int_Z.succ_big_int (Big_int_Z.succ_big_int
-    (Big_int_Z.succ_big_int (Big_int_Z.succ_big_int (Big_int_Z.succ_big_int
-    (Big_int_Z.succ_big_int (Big_int_Z.succ_big_int (Big_int_Z.succ_big_int
-    (Big_int_Z.succ_big_int (Big_int_Z.succ_big_int (Big_int_Z.succ_big_int
-    (Big_int_Z.succ_big_int (Big_int_Z.succ_big_int (Big_int_Z.succ_big_int
-    (Big_int_Z.succ_big_int (Big_int_Z.succ_big_int (Big_int_Z.succ_big_int
-    (Big_int_Z.succ_big_int (Big_int_Z.succ_big_int (Big_int_Z.succ_big_int
-    (Big_int_Z.succ_big_int (Big_int_Z.succ_big_int
-    Big_int_Z.zero_big_int))))))))))))))))))))))))))))))))))))))))))))))))))))))))))))))))))))))
-
-(** val eRR_AXS_BAD_C : Big_int_Z.big_int **)
-
-let eRR_AXS_BAD_C =
-  Big_int_Z.succ_big_int (Big_int_Z.succ_big_int (Big_int_Z.succ_big_int
-    (Big_int_Z.succ_big_int (Big_int_Z.succ_big_int (Big_int_Z.succ_big_int
-    (Big_int_Z.succ_big_int (Big_int_Z.succ_big_int (Big_int_Z.succ_big_int
-    (Big_int_Z.succ_big_int (Big_int_Z.succ_big_int (Big_int_Z.succ_big_int
-    (Big_int_Z.succ_big_int (Big_int_Z.succ_big_int (Big_int_Z.succ_big_int
-    (Big_int_Z.succ_big_int (Big_int_Z.succ_big_int (Big_int_Z.succ_big_int
-    (Big_int_Z.succ_big_int (Big_int_Z.succ_big_int (Big_int_Z.succ_big_int
-    (Big_int_Z.succ_big_int (Big_int_Z.succ_big_int (Big_int_Z.succ_big_int
-    (Big_int_Z.succ_big_int (Big_int_Z.succ_big_int (Big_int_Z.succ_big_int
-    (Big_int_Z.succ_big_int (Big_int_Z.succ_big_int (Big_int_Z.succ_big_int
-    (Big_int_Z.succ_big_int (Big_int_Z.succ_big_int (Big_int_Z.succ_big_int
-    (Big_int_Z.succ_big_int (Big_int_Z.succ_big_int (Big_int_Z.succ_big_int
-    (Big_int_Z.succ_big_int (Big_int_Z.succ_big_int (Big_int_Z.succ_big_int
-    (Big_int_Z.succ_big_int (Big_int_Z.succ_big_int (Big_int_Z.succ_big_int
-    (Big_int_Z.succ_big_int (Big_int_Z.succ_big_int (Big_int_Z.succ_big_int
-    (Big_int_Z.succ_big_int (Big_int_Z.succ_big_int (Big_int_Z.succ_big_int
-    (Big_int_Z.succ_big_int (Big_int_Z.succ_big_int (Big_int_Z.succ_big_int
-    (Big_int_Z.succ_big_int (Big_int_Z.succ_big_int (Big_int_Z.succ_big_int
-    (Big_int_Z.succ_big_int (Big_int_Z.succ_big_int (Big_int_Z.succ_big_int
-    (Big_int_Z.succ_big_int (Big_int_Z.succ_big_int (Big_int_Z.succ_big_int
-    (Big_int_Z.succ_big_int (Big_int_Z.succ_big_int (Big_int_Z.succ_big_int
-    (Big_int_Z.succ_big_int (Big_int_Z.succ_big_int (Big_int_Z.succ_big_int
-    (Big_int_Z.succ_big_int (Big_int_Z.succ_big_int (Big_int_Z.succ_big_int
-    (Big_int_Z.succ_big_int (Big_int_Z.succ_big_int (Big_int_Z.succ_big_int
-    Big_int_Z.zero_big_int)))))))))))))))))))))))))))))))))))))))))))))))))))))))))))))))))))))))
-
-(** val eRR_MP_P_NOT_LT_J : Big_int_Z.big_int **)
-
-let eRR_MP_P_NOT_LT_J =
-  Big_int_Z.succ_big_int (Big_int_Z.succ_big_int (Big_int_Z.succ_big_int
-    (Big_int_Z.succ_big_int (Big_int_Z.succ_big_int (Big_int_Z.succ_big_int
-    (Big_int_Z.succ_big_int (Big_int_Z.succ_big_int (Big_int_Z.succ_big_int
-    (Big_int_Z.succ_big_int (Big_int_Z.succ_big_int (Big_int_Z.succ_big_int
-    (Big_int_Z.succ_big_int (Big_int_Z.succ_big_int (Big_int_Z.succ_big_int
-    (Big_int_Z.succ_big_int (Big_int_Z.succ_big_int (Big_int_Z.succ_big_int
-    (Big_int_Z.succ_big_int (Big_int_Z.succ_big_int (Big_int_Z.succ_big_int
-    (Big_int_Z.succ_big_int (Big_int_Z.succ_big_int (Big_int_Z.succ_big_int
-    (Big_int_Z.succ_big_int (Big_int_Z.succ_big_int (Big_int_Z.succ_big_int
-    (Big_int_Z.succ_big_int (Big_int_Z.succ_big_int (Big_int_Z.succ_big_int
-    (Big_int_Z.succ_big_int (Big_int_Z.succ_big_int (Big_int_Z.succ_big_int
-    (Big_int_Z.succ_big_int (Big_int_Z.succ_big_int (Big_int_Z.succ_big_int
-    (Big_int_Z.succ_big_int (Big_int_Z.succ_big_int (Big_int_Z.succ_big_int
-    (Big_int_Z.succ_big_int (Big_int_Z.succ_big_int (Big_int_Z.succ_big_int
-    (Big_int_Z.succ_big_int (Big_int_Z.succ_big_int (Big_int_Z.succ_big_int
-    (Big_int_Z.succ_big_int (Big_int_Z.succ_big_int (Big_int_Z.succ_big_int
-    (Big_int_Z.succ_big_int (Big_int_Z.succ_big_int (Big_int_Z.succ_big_int
-    (Big_int_Z.succ_big_int (Big_int_Z.succ_big_int (Big_int_Z.succ_big_int
-    (Big_int_Z.succ_big_int (Big_int_Z.succ_big_int (Big_int_Z.succ_big_int
-    (Big_int_Z.succ_big_int (Big_int_Z.succ_big_int (Big_int_Z.succ_big_int
-    (Big_int_Z.succ_big_int (Big_int_Z.succ_big_int (Big_int_Z.succ_big_int
-    (Big_int_Z.succ_big_int (Big_int_Z.succ_big_int (Big_int_Z.succ_big_int
-    (Big_int_Z.succ_big_int (Big_int_Z.succ_big_int (Big_int_Z.succ_big_int
-    (Big_int_Z.succ_big_int (Big_int_Z.succ_big_int (Big_int_Z.succ_big_int
-    (Big_int_Z.succ_big_int (Big_int_Z.succ_big_int (Big_int_Z.succ_big_int
-    (Big_int_Z.succ_big_int (Big_int_Z.succ_big_int (Big_int_Z.succ_big_int
-    (Big_int_Z.succ_big_int (Big_int_Z.succ_big_int (Big_int_Z.succ_big_int
-    (Big_int_Z.succ_big_int (Big_int_Z.succ_big_int (Big_int_Z.succ_big_int
-    (Big_int_Z.succ_big_int (Big_int_Z.succ_big_int (Big_int_Z.succ_big_int
-    (Big_int_Z.succ_big_int (Big_int_Z.succ_big_int (Big_int_Z.succ_big_int
-    (Big_int_Z.succ_big_int (Big_int_Z.succ_big_int
-    Big_int_Z.zero_big_int)))))))))))))))))))))))))))))))))))))))))))))))))))))))))))))))))))))))))))))))))))))))))))
-
-(** val eRR_MP_Q_NOT_LT_J : Big_int_Z.big_int **)
-
-let eRR_MP_Q_NOT_LT_J =
-  Big_int_Z.succ_big_int (Big_int_Z.succ_big_int (Big_int_Z.succ_big_int
-    (Big_int_Z.succ_big_int (Big_int_Z.succ_big_int (Big_int_Z.succ_big_int
-    (Big_int_Z.succ_big_int (Big_int_Z.succ_big_int (Big_int_Z.succ_big_int
-    (Big_int_Z.succ_big_int (Big_int_Z.succ_big_int (Big_int_Z.succ_big_int
-    (Big_int_Z.succ_big_int (Big_int_Z.succ_big_int (Big_int_Z.succ_big_int
-    (Big_int_Z.succ_big_int (Big_int_Z.succ_big_int (Big_int_Z.succ_big_int
-    (Big_int_Z.succ_big_int (Big_int_Z.succ_big_int (Big_int_Z.succ_big_int
-    (Big_int_Z.succ_big_int (Big_int_Z.succ_big_int (Big_int_Z.succ_big_int
-    (Big_int_Z.succ_big_int (Big_int_Z.succ_big_int (Big_int_Z.succ_big_int
-    (Big_int_Z.succ_big_int (Big_int_Z.succ_big_int (Big_int_Z.succ_big_int
-    (Big_int_Z.succ_big_int (Big_int_Z.succ_big_int (Big_int_Z.succ_big_int
-    (Big_int_Z.succ_big_int (Big_int_Z.succ_big_int (Big_int_Z.succ_big_int
-    (Big_int_Z.succ_big_int (Big_int_Z.succ_big_int (Big_int_Z.succ_big_int
-    (Big_int_Z.succ_big_int (Big_int_Z.succ_big_int (Big_int_Z.succ_big_int
-    (Big_int_Z.succ_big_int (Big_int_Z.succ_big_int (Big_int_Z.succ_big_int
-    (Big_int_Z.succ_big_int (Big_int_Z.succ_big_int (Big_int_Z.succ_big_int
-    (Big_int_Z.succ_big_int (Big_int_Z.succ_big_int (Big_int_Z.succ_big_int
-    (Big_int_Z.succ_big_int (Big_int_Z.succ_big_int (Big_int_Z.succ_big_int
-    (Big_int_Z.succ_big_int (Big_int_Z.succ_big_int (Big_int_Z.succ_big_int
-    (Big_int_Z.succ_big_int (Big_int_Z.succ_big_int (Big_int_Z.succ_big_int
-    (Big_int_Z.succ_big_int (Big_int_Z.succ_big_int (Big_int_Z.succ_big_int
-    (Big_int_Z.succ_big_int (Big_int_Z.succ_big_int (Big_int_Z.succ_big_int
-    (Big_int_Z.succ_big_int (Big_int_Z.succ_big_int (Big_int_Z.succ_big_int
-    (Big_int_Z.succ_big_int (Big_int_Z.succ_big_int (Big_int_Z.succ_big_int
-    (Big_int_Z.succ_big_int (Big_int_Z.succ_big_int (Big_int_Z.succ_big_int
-    (Big_int_Z.succ_big_int (Big_int_Z.succ_big_int (Big_int_Z.succ_big_int
-    (Big_int_Z.succ_big_int (Big_int_Z.succ_big_int (Big_int_Z.succ_big_int
-    (Big_int_Z.succ_big_int (Big_int_Z.succ_big_int (Big_int_Z.succ_big_int
-    (Big_int_Z.succ_big_int (Big_int_Z.succ_big_int (Big_int_Z.succ_big_int
-    (Big_int_Z.succ_big_int (Big_int_Z.succ_big_int (Big_int_Z.succ_big_int
-    (Big_int_Z.succ_big_int (Big_int_Z.succ_big_int (Big_int_Z.succ_big_int
-    Big_int_Z.zero_big_int))))))))))))))))))))))))))))))))))))))))))))))))))))))))))))))))))))))))))))))))))))))))))))
-
-(** val eRR_MP_BAD_LINE_J : Big_int_Z.big_int **)
-
-let eRR_MP_BAD_LINE_J =
-  Big_int_Z.succ_big_int (Big_int_Z.succ_big_int (Big_int_Z.succ_big_int
-    (Big_int_Z.succ_big_int (Big_int_Z.succ_big_int (Big_int_Z.succ_big_int
-    (Big_int_Z.succ_big_int (Big_int_Z.succ_big_int (Big_int_Z.succ_big_int
-    (Big_int_Z.succ_big_int (Big_int_Z.succ_big_int (Big_int_Z.succ_big_int
-    (Big_int_Z.succ_big_int (Big_int_Z.succ_big_int (Big_int_Z.succ_big_int
-    (Big_int_Z.succ_big_int (Big_int_Z.succ_big_int (Big_int_Z.succ_big_int
-    (Big_int_Z.succ_big_int (Big_int_Z.succ_big_int (Big_int_Z.succ_big_int
-    (Big_int_Z.succ_big_int (Big_int_Z.succ_big_int (Big_int_Z.succ_big_int
-    (Big_int_Z.succ_big_int (Big_int_Z.succ_big_int (Big_int_Z.succ_big_int
-    (Big_int_Z.succ_big_int (Big_int_Z.succ_big_int (Big_int_Z.succ_big_int
-    (Big_int_Z.succ_big_int (Big_int_Z.succ_big_int (Big_int_Z.succ_big_int
-    (Big_int_Z.succ_big_int (Big_int_Z.succ_big_int (Big_int_Z.succ_big_int
-    (Big_int_Z.succ_big_int (Big_int_Z.succ_big_int (Big_int_Z.succ_big_int
-    (Big_int_Z.succ_big_int (Big_int_Z.succ_big_int (Big_int_Z.succ_big_int
-    (Big_int_Z.succ_big_int (Big_int_Z.succ_big_int (Big_int_Z.succ_big_int
-    (Big_int_Z.succ_big_int (Big_int_Z.succ_big_int (Big_int_Z.succ_big_int
-    (Big_int_Z.succ_big_int (Big_int_Z.succ_big_int (Big_int_Z.succ_big_int
-    (Big_int_Z.succ_big_int (Big_int_Z.succ_big_int (Big_int_Z.succ_big_int
-    (Big_int_Z.succ_big_int (Big_int_Z.succ_big_int (Big_int_Z.succ_big_int
-    (Big_int_Z.succ_big_int (Big_int_Z.succ_big_int (Big_int_Z.succ_big_int
-    (Big_int_Z.succ_big_int (Big_int_Z.succ_big_int (Big_int_Z.succ_big_int
-    (Big_int_Z.succ_big_int (Big_int_Z.succ_big_int (Big_int_Z.succ_big_int
-    (Big_int_Z.succ_big_int (Big_int_Z.succ_big_int (Big_int_Z.succ_big_int
-    (Big_int_Z.succ_big_int (Big_int_Z.succ_big_int (Big_int_Z.succ_big_int
-    (Big_int_Z.succ_big_int (Big_int_Z.succ_big_int (Big_int_Z.succ_big_int
-    (Big_int_Z.succ_big_int (Big_int_Z.succ_big_int (Big_int_Z.succ_big_int
-    (Big_int_Z.succ_big_int (Big_int_Z.succ_big_int (Big_int_Z.succ_big_int
-    (Big_int_Z.succ_big_int (Big_int_Z.succ_big_int (Big_int_Z.succ_big_int
-    (Big_int_Z.succ_big_int (Big_int_Z.succ_big_int (Big_int_Z.succ_big_int
-    (Big_int_Z.succ_big_int (Big_int_Z.succ_big_int (Big_int_Z.succ_big_int
-    (Big_int_Z.succ_big_int (Big_int_Z.succ_big_int (Big_int_Z.succ_big_int
-    (Big_int_Z.succ_big_int
-    Big_int_Z.zero_big_int)))))))))))))))))))))))))))))))))))))))))))))))))))))))))))))))))))))))))))))))))))))))))))))
-
-(** val eRR_MP_BAD_LINE_P : Big_int_Z.big_int **)
-
-let eRR_MP_BAD_LINE_P =
-  Big_int_Z.succ_big_int (Big_int_Z.succ_big_int (Big_int_Z.succ_big_int
-    (Big_int_Z.succ_big_int (Big_int_Z.succ_big_int (Big_int_Z.succ_big_int
-    (Big_int_Z.succ_big_int (Big_int_Z.succ_big_int (Big_int_Z.succ_big_int
-    (Big_int_Z.succ_big_int (Big_int_Z.succ_big_int (Big_int_Z.succ_big_int
-    (Big_int_Z.succ_big_int (Big_int_Z.succ_big_int (Big_int_Z.succ_big_int
-    (Big_int_Z.succ_big_int (Big_int_Z.succ_big_int (Big_int_Z.succ_big_int
-    (Big_int_Z.succ_big_int (Big_int_Z.succ_big_int (Big_int_Z.succ_big_int
-    (Big_int_Z.succ_big_int (Big_int_Z.succ_big_int (Big_int_Z.succ_big_int
-    (Big_int_Z.succ_big_int (Big_int_Z.succ_big_int (Big_int_Z.succ_big_int
-    (Big_int_Z.succ_big_int (Big_int_Z.succ_big_int (Big_int_Z.succ_big_int
-    (Big_int_Z.succ_big_int (Big_int_Z.succ_big_int (Big_int_Z.succ_big_int
-    (Big_int_Z.succ_big_int (Big_int_Z.succ_big_int (Big_int_Z.succ_big_int
-    (Big_int_Z.succ_big_int (Big_int_Z.succ_big_int (Big_int_Z.succ_big_int
-    (Big_int_Z.succ_big_int (Big_int_Z.succ_big_int (Big_int_Z.succ_big_int
-    (Big_int_Z.succ_big_int (Big_int_Z.succ_big_int (Big_int_Z.succ_big_int
-    (Big_int_Z.succ_big_int (Big_int_Z.succ_big_int (Big_int_Z.succ_big_int
-    (Big_int_Z.succ_big_int (Big_int_Z.succ_big_int (Big_int_Z.succ_big_int
-    (Big_int_Z.succ_big_int (Big_int_Z.succ_big_int (Big_int_Z.succ_big_int
-    (Big_int_Z.succ_big_int (Big_int_Z.succ_big_int (Big_int_Z.succ_big_int
-    (Big_int_Z.succ_big_int (Big_int_Z.succ_big_int (Big_int_Z.succ_big_int
-    (Big_int_Z.succ_big_int (Big_int_Z.succ_big_int (Big_int_Z.succ_big_int
-    (Big_int_Z.succ_big_int (Big_int_Z.succ_big_int (Big_int_Z.succ_big_int
-    (Big_int_Z.succ_big_int (Big_int_Z.succ_big_int (Big_int_Z.succ_big_int
-    (Big_int_Z.succ_big_int (Big_int_Z.succ_big_int (Big_int_Z.succ_big_int
-    (Big_int_Z.succ_big_int (Big_int_Z.succ_big_int (Big_int_Z.succ_big_int
-    (Big_int_Z.succ_big_int (Big_int_Z.succ_big_int (Big_int_Z.succ_big_int
-    (Big_int_Z.succ_big_int (Big_int_Z.succ_big_int (Big_int_Z.succ_big_int
-    (Big_int_Z.succ_big_int (Big_int_Z.succ_big_int (Big_int_Z.succ_big_int
-    (Big_int_Z.succ_big_int (Big_int_Z.succ_big_int (Big_int_Z.succ_big_int
-    (Big_int_Z.succ_big_int (Big_int_Z.succ_big_int (Big_int_Z.succ_big_int
-    (Big_int_Z.succ_big_int (Big_int_Z.succ_big_int (Big_int_Z.succ_big_int
-    (Big_int_Z.succ_big_int (Big_int_Z.succ_big_int
-    Big_int_Z.zero_big_int))))))))))))))))))))))))))))))))))))))))))))))))))))))))))))))))))))))))))))))))))))))))))))))
-
-(** val eRR_MP_BAD_LINE_Q : Big_int_Z.big_int **)
-
-let eRR_MP_BAD_LINE_Q =
-  Big_int_Z.succ_big_int (Big_int_Z.succ_big_int (Big_int_Z.succ_big_int
-    (Big_int_Z.succ_big_int (Big_int_Z.succ_big_int (Big_int_Z.succ_big_int
-    (Big_int_Z.succ_big_int (Big_int_Z.succ_big_int (Big_int_Z.succ_big_int
-    (Big_int_Z.succ_big_int (Big_int_Z.succ_big_int (Big_int_Z.succ_big_int
-    (Big_int_Z.succ_big_int (Big_int_Z.succ_big_int (Big_int_Z.succ_big_int
-    (Big_int_Z.succ_big_int (Big_int_Z.succ_big_int (Big_int_Z.succ_big_int
-    (Big_int_Z.succ_big_int (Big_int_Z.succ_big_int (Big_int_Z.succ_big_int
-    (Big_int_Z.succ_big_int (Big_int_Z.succ_big_int (Big_int_Z.succ_big_int
-    (Big_int_Z.succ_big_int (Big_int_Z.succ_big_int (Big_int_Z.succ_big_int
-    (Big_int_Z.succ_big_int (Big_int_Z.succ_big_int (Big_int_Z.succ_big_int
-    (Big_int_Z.succ_big_int (Big_int_Z.succ_big_int (Big_int_Z.succ_big_int
-    (Big_int_Z.succ_big_int (Big_int_Z.succ_big_int (Big_int_Z.succ_big_int
-    (Big_int_Z.succ_big_int (Big_int_Z.succ_big_int (Big_int_Z.succ_big_int
-    (Big_int_Z.succ_big_int (Big_int_Z.succ_big_int (Big_int_Z.succ_big_int
-    (Big_int_Z.succ_big_int (Big_int_Z.succ_big_int (Big_int_Z.succ_big_int
-    (Big_int_Z.succ_big_int (Big_int_Z.succ_big_int (Big_int_Z.succ_big_int
-    (Big_int_Z.succ_big_int (Big_int_Z.succ_big_int (Big_int_Z.succ_big_int
-    (Big_int_Z.succ_big_int (Big_int_Z.succ_big_int (Big_int_Z.succ_big_int
-    (Big_int_Z.succ_big_int (Big_int_Z.succ_big_int (Big_int_Z.succ_big_int
-    (Big_int_Z.succ_big_int (Big_int_Z.succ_big_int (Big_int_Z.succ_big_int
-    (Big_int_Z.succ_big_int (Big_int_Z.succ_big_int (Big_int_Z.succ_big_int
-    (Big_int_Z.succ_big_int (Big_int_Z.succ_big_int (Big_int_Z.succ_big_int
-    (Big_int_Z.succ_big_int (Big_int_Z.succ_big_int (Big_int_Z.succ_big_int
-    (Big_int_Z.succ_big_int (Big_int_Z.succ_big_int (Big_int_Z.succ_big_int
-    (Big_int_Z.succ_big_int (Big_int_Z.succ_big_int (Big_int_Z.succ_big_int
-    (Big_int_Z.succ_big_int (Big_int_Z.succ_big_int (Big_int_Z.succ_big_int
-    (Big_int_Z.succ_big_int (Big_int_Z.succ_big_int (Big_int_Z.succ_big_int
-    (Big_int_Z.succ_big_int (Big_int_Z.succ_big_int (Big_int_Z.succ_big_int
-    (Big_int_Z.succ_big_int (Big_int_Z.succ_big_int (Big_int_Z.succ_big_int
-    (Big_int_Z.succ_big_int (Big_int_Z.succ_big_int (Big_int_Z.succ_big_int
-    (Big_int_Z.succ_big_int (Big_int_Z.succ_big_int (Big_int_Z.succ_big_int
-    (Big_int_Z.succ_big_int (Big_int_Z.succ_big_int (Big_int_Z.succ_big_int
-    Big_int_Z.zero_big_int)))))))))))))))))))))))))))))))))))))))))))))))))))))))))))))))))))))))))))))))))))))))))))))))
-
-(** val eRR_MP_Q_NOT_IMP : Big_int_Z.big_int **)
-
-let eRR_MP_Q_NOT_IMP =
-  Big_int_Z.succ_big_int (Big_int_Z.succ_big_int (Big_int_Z.succ_big_int
-    (Big_int_Z.succ_big_int (Big_int_Z.succ_big_int (Big_int_Z.succ_big_int
-    (Big_int_Z.succ_big_int (Big_int_Z.succ_big_int (Big_int_Z.succ_big_int
-    (Big_int_Z.succ_big_int (Big_int_Z.succ_big_int (Big_int_Z.succ_big_int
-    (Big_int_Z.succ_big_int (Big_int_Z.succ_big_int (Big_int_Z.succ_big_int
-    (Big_int_Z.succ_big_int (Big_int_Z.succ_big_int (Big_int_Z.succ_big_int
-    (Big_int_Z.succ_big_int (Big_int_Z.succ_big_int (Big_int_Z.succ_big_int
-    (Big_int_Z.succ_big_int (Big_int_Z.succ_big_int (Big_int_Z.succ_big_int
-    (Big_int_Z.succ_big_int (Big_int_Z.succ_big_int (Big_int_Z.succ_big_int
-    (Big_int_Z.succ_big_int (Big_int_Z.succ_big_int (Big_int_Z.succ_big_int
-    (Big_int_Z.succ_big_int (Big_int_Z.succ_big_int (Big_int_Z.succ_big_int
-    (Big_int_Z.succ_big_int (Big_int_Z.succ_big_int (Big_int_Z.succ_big_int
-    (Big_int_Z.succ_big_int (Big_int_Z.succ_big_int (Big_int_Z.succ_big_int
-    (Big_int_Z.succ_big_int (Big_int_Z.succ_big_int (Big_int_Z.succ_big_int
-    (Big_int_Z.succ_big_int (Big_int_Z.succ_big_int (Big_int_Z.succ_big_int
-    (Big_int_Z.succ_big_int (Big_int_Z.succ_big_int (Big_int_Z.succ_big_int
-    (Big_int_Z.succ_big_int (Big_int_Z.succ_big_int (Big_int_Z.succ_big_int
-    (Big_int_Z.succ_big_int (Big_int_Z.succ_big_int (Big_int_Z.succ_big_int
-    (Big_int_Z.succ_big_int (Big_int_Z.succ_big_int (Big_int_Z.succ_big_int
-    (Big_int_Z.succ_big_int (Big_int_Z.succ_big_int (Big_int_Z.succ_big_int
-    (Big_int_Z.succ_big_int (Big_int_Z.succ_big_int (Big_int_Z.succ_big_int
-    (Big_int_Z.succ_big_int (Big_int_Z.succ_big_int (Big_int_Z.succ_big_int
-    (Big_int_Z.succ_big_int (Big_int_Z.succ_big_int (Big_int_Z.succ_big_int
-    (Big_int_Z.succ_big_int (Big_int_Z.succ_big_int (Big_int_Z.succ_big_int
-    (Big_int_Z.succ_big_int (Big_int_Z.succ_big_int (Big_int_Z.succ_big_int
-    (Big_int_Z.succ_big_int (Big_int_Z.succ_big_int (Big_int_Z.succ_big_int
-    (Big_int_Z.succ_big_int (Big_int_Z.succ_big_int (Big_int_Z.succ_big_int
-    (Big_int_Z.succ_big_int (Big_int_Z.succ_big_int (Big_int_Z.succ_big_int
-    (Big_int_Z.succ_big_int (Big_int_Z.succ_big_int (Big_int_Z.succ_big_int
-    (Big_int_Z.succ_big_int (Big_int_Z.succ_big_int (Big_int_Z.succ_big_int
-    (Big_int_Z.succ_big_int (Big_int_Z.succ_big_int (Big_int_Z.succ_big_int
-    (Big_int_Z.succ_big_int (Big_int_Z.succ_big_int (Big_int_Z.succ_big_int
-    (Big_int_Z.succ_big_int
-    Big_int_Z.zero_big_int))))))))))))))))))))))))))))))))))))))))))))))))))))))))))))))))))))))))))))))))))))))))))))))))
-
-(** val eRR_MP_ANTECEDENT_MISMATCH : Big_int_Z.big_int **)
-
-let eRR_MP_ANTECEDENT_MISMATCH =
-  Big_int_Z.succ_big_int (Big_int_Z.succ_big_int (Big_int_Z.succ_big_int
-    (Big_int_Z.succ_big_int (Big_int_Z.succ_big_int (Big_int_Z.succ_big_int
-    (Big_int_Z.succ_big_int (Big_int_Z.succ_big_int (Big_int_Z.succ_big_int
-    (Big_int_Z.succ_big_int (Big_int_Z.succ_big_int (Big_int_Z.succ_big_int
-    (Big_int_Z.succ_big_int (Big_int_Z.succ_big_int (Big_int_Z.succ_big_int
-    (Big_int_Z.succ_big_int (Big_int_Z.succ_big_int (Big_int_Z.succ_big_int
-    (Big_int_Z.succ_big_int (Big_int_Z.succ_big_int (Big_int_Z.succ_big_int
-    (Big_int_Z.succ_big_int (Big_int_Z.succ_big_int (Big_int_Z.succ_big_int
-    (Big_int_Z.succ_big_int (Big_int_Z.succ_big_int (Big_int_Z.succ_big_int
-    (Big_int_Z.succ_big_int (Big_int_Z.succ_big_int (Big_int_Z.succ_big_int
-    (Big_int_Z.succ_big_int (Big_int_Z.succ_big_int (Big_int_Z.succ_big_int
-    (Big_int_Z.succ_big_int (Big_int_Z.succ_big_int (Big_int_Z.succ_big_int
-    (Big_int_Z.succ_big_int (Big_int_Z.succ_big_int (Big_int_Z.succ_big_int
-    (Big_int_Z.succ_big_int (Big_int_Z.succ_big_int (Big_int_Z.succ_big_int
-    (Big_int_Z.succ_big_int (Big_int_Z.succ_big_int (Big_int_Z.succ_big_int
-    (Big_int_Z.succ_big_int (Big_int_Z.succ_big_int (Big_int_Z.succ_big_int
-    (Big_int_Z.succ_big_int (Big_int_Z.succ_big_int (Big_int_Z.succ_big_int
-    (Big_int_Z.succ_big_int (Big_int_Z.succ_big_int (Big_int_Z.succ_big_int
-    (Big_int_Z.succ_big_int (Big_int_Z.succ_big_int (Big_int_Z.succ_big_int
-    (Big_int_Z.succ_big_int (Big_int_Z.succ_big_int (Big_int_Z.succ_big_int
-    (Big_int_Z.succ_big_int (Big_int_Z.succ_big_int (Big_int_Z.succ_big_int
-    (Big_int_Z.succ_big_int (Big_int_Z.succ_big_int (Big_int_Z.succ_big_int
-    (Big_int_Z.succ_big_int (Big_int_Z.succ_big_int (Big_int_Z.succ_big_int
-    (Big_int_Z.succ_big_int (Big_int_Z.succ_big_int (Big_int_Z.succ_big_int
-    (Big_int_Z.succ_big_int (Big_int_Z.succ_big_int (Big_int_Z.succ_big_int
-    (Big_int_Z.succ_big_int (Big_int_Z.succ_big_int (Big_int_Z.succ_big_int
-    (Big_int_Z.succ_big_int (Big_int_Z.succ_big_int (Big_int_Z.succ_big_int
-    (Big_int_Z.succ_big_int (Big_int_Z.succ_big_int (Big_int_Z.succ_big_int
-    (Big_int_Z.succ_big_int (Big_int_Z.succ_big_int (Big_int_Z.succ_big_int
-    (Big_int_Z.succ_big_int (Big_int_Z.succ_big_int (Big_int_Z.succ_big_int
-    (Big_int_Z.succ_big_int (Big_int_Z.succ_big_int (Big_int_Z.succ_big_int
-    (Big_int_Z.succ_big_int (Big_int_Z.succ_big_int (Big_int_Z.succ_big_int
-    (Big_int_Z.succ_big_int (Big_int_Z.succ_big_int
-    Big_int_Z.zero_big_int)))))))))))))))))))))))))))))))))))))))))))))))))))))))))))))))))))))))))))))))))))))))))))))))))
-
-(** val eRR_MP_CONSEQUENT_MISMATCH : Big_int_Z.big_int **)
-
-let eRR_MP_CONSEQUENT_MISMATCH =
-  Big_int_Z.succ_big_int (Big_int_Z.succ_big_int (Big_int_Z.succ_big_int
-    (Big_int_Z.succ_big_int (Big_int_Z.succ_big_int (Big_int_Z.succ_big_int
-    (Big_int_Z.succ_big_int (Big_int_Z.succ_big_int (Big_int_Z.succ_big_int
-    (Big_int_Z.succ_big_int (Big_int_Z.succ_big_int (Big_int_Z.succ_big_int
-    (Big_int_Z.succ_big_int (Big_int_Z.succ_big_int (Big_int_Z.succ_big_int
-    (Big_int_Z.succ_big_int (Big_int_Z.succ_big_int (Big_int_Z.succ_big_int
-    (Big_int_Z.succ_big_int (Big_int_Z.succ_big_int (Big_int_Z.succ_big_int
-    (Big_int_Z.succ_big_int (Big_int_Z.succ_big_int (Big_int_Z.succ_big_int
-    (Big_int_Z.succ_big_int (Big_int_Z.succ_big_int (Big_int_Z.succ_big_int
-    (Big_int_Z.succ_big_int (Big_int_Z.succ_big_int (Big_int_Z.succ_big_int
-    (Big_int_Z.succ_big_int (Big_int_Z.succ_big_int (Big_int_Z.succ_big_int
-    (Big_int_Z.succ_big_int (Big_int_Z.succ_big_int (Big_int_Z.succ_big_int
-    (Big_int_Z.succ_big_int (Big_int_Z.succ_big_int (Big_int_Z.succ_big_int
-    (Big_int_Z.succ_big_int (Big_int_Z.succ_big_int (Big_int_Z.succ_big_int
-    (Big_int_Z.succ_big_int (Big_int_Z.succ_big_int (Big_int_Z.succ_big_int
-    (Big_int_Z.succ_big_int (Big_int_Z.succ_big_int (Big_int_Z.succ_big_int
-    (Big_int_Z.succ_big_int (Big_int_Z.succ_big_int (Big_int_Z.succ_big_int
-    (Big_int_Z.succ_big_int (Big_int_Z.succ_big_int (Big_int_Z.succ_big_int
-    (Big_int_Z.succ_big_int (Big_int_Z.succ_big_int (Big_int_Z.succ_big_int
-    (Big_int_Z.succ_big_int (Big_int_Z.succ_big_int (Big_int_Z.succ_big_int
-    (Big_int_Z.succ_big_int (Big_int_Z.succ_big_int (Big_int_Z.succ_big_int
-    (Big_int_Z.succ_big_int (Big_int_Z.succ_big_int (Big_int_Z.succ_big_int
-    (Big_int_Z.succ_big_int (Big_int_Z.succ_big_int (Big_int_Z.succ_big_int
-    (Big_int_Z.succ_big_int (Big_int_Z.succ_big_int (Big_int_Z.succ_big_int
-    (Big_int_Z.succ_big_int (Big_int_Z.succ_big_int (Big_int_Z.succ_big_int
-    (Big_int_Z.succ_big_int (Big_int_Z.succ_big_int (Big_int_Z.succ_big_int
-    (Big_int_Z.succ_big_int (Big_int_Z.succ_big_int (Big_int_Z.succ_big_int
-    (Big_int_Z.succ_big_int (Big_int_Z.succ_big_int (Big_int_Z.succ_big_int
-    (Big_int_Z.succ_big_int (Big_int_Z.succ_big_int (Big_int_Z.succ_big_int
-    (Big_int_Z.succ_big_int (Big_int_Z.succ_big_int (Big_int_Z.succ_big_int
-    (Big_int_Z.succ_big_int (Big_int_Z.succ_big_int (Big_int_Z.succ_big_int
-    (Big_int_Z.succ_big_int (Big_int_Z.succ_big_int (Big_int_Z.succ_big_int
-    (Big_int_Z.succ_big_int (Big_int_Z.succ_big_int (Big_int_Z.succ_big_int
-    Big_int_Z.zero_big_int))))))))))))))))))))))))))))))))))))))))))))))))))))))))))))))))))))))))))))))))))))))))))))))))))
 
 (** val fst001 : Big_int_Z.big_int -> Big_int_Z.big_int **)
 
@@ -1306,17 +516,6 @@ let tAG_NIL =
 let tAG_CONS =
   Big_int_Z.succ_big_int Big_int_Z.zero_big_int
 
-(** val code_nil : Big_int_Z.big_int **)
-
-let code_nil =
-  encode tAG_NIL Big_int_Z.zero_big_int
-
-(** val code_cons :
-    Big_int_Z.big_int -> Big_int_Z.big_int -> Big_int_Z.big_int **)
-
-let code_cons h t =
-  encode tAG_CONS (encode h t)
-
 (** val list_tag : Big_int_Z.big_int -> Big_int_Z.big_int **)
 
 let list_tag =
@@ -1331,55 +530,6 @@ let list_payload =
 
 let is_nil_nodeb body =
   is_pair001b body tAG_NIL Big_int_Z.zero_big_int
-
-(** val cons_payloadb : Big_int_Z.big_int -> bool **)
-
-let cons_payloadb =
-  canonical001b
-
-(** val list_exact_lengthb :
-    Big_int_Z.big_int -> Big_int_Z.big_int -> bool **)
-
-let rec list_exact_lengthb n body =
-  (fun fO fS n -> if Big_int_Z.sign_big_int n <= 0 then fO ()
-  else fS (Big_int_Z.pred_big_int n))
-    (fun _ -> is_nil_nodeb body)
-    (fun n' ->
-    if canonical001b body
-    then if Nat.eqb (list_tag body) tAG_CONS
-         then let payload = list_payload body in
-              if cons_payloadb payload
-              then list_exact_lengthb n' (snd001 payload)
-              else false
-         else false
-    else false)
-    n
-
-(** val nth_list_fuel :
-    Big_int_Z.big_int -> Big_int_Z.big_int -> Big_int_Z.big_int ->
-    Big_int_Z.big_int **)
-
-let rec nth_list_fuel fuel body i =
-  (fun fO fS n -> if Big_int_Z.sign_big_int n <= 0 then fO ()
-  else fS (Big_int_Z.pred_big_int n))
-    (fun _ -> reject sTAGE_LIST_STRUCTURE i eRR_FUEL_EXHAUSTED)
-    (fun fuel' ->
-    if canonical001b body
-    then let tag = list_tag body in
-         let payload = list_payload body in
-         if Nat.eqb tag tAG_CONS
-         then if cons_payloadb payload
-              then let h = fst001 payload in
-                   let t = snd001 payload in
-                   if Nat.eqb i Big_int_Z.zero_big_int
-                   then accept h
-                   else nth_list_fuel fuel' t (Nat.pred i)
-              else reject sTAGE_LIST_STRUCTURE i eRR_NONCANONICAL_NODE
-         else if Nat.eqb tag tAG_NIL
-              then reject sTAGE_LIST_STRUCTURE i eRR_INDEX_OUT_OF_RANGE
-              else reject sTAGE_LIST_STRUCTURE i eRR_BAD_LIST_TAG
-    else reject sTAGE_LIST_STRUCTURE i eRR_NONCANONICAL_NODE)
-    fuel
 
 (** val tAG_VAR : Big_int_Z.big_int **)
 
@@ -1431,20 +581,6 @@ let formula_bound c =
 
 let is_formula c =
   is_formula_fuel (formula_bound c) c
-
-(** val parse_imp : Big_int_Z.big_int -> Big_int_Z.big_int **)
-
-let parse_imp phi =
-  if canonical001b phi
-  then let tag = formula_tag phi in
-       let payload = formula_payload phi in
-       if Nat.eqb tag tAG_IMP
-       then if canonical001b payload
-            then accept payload
-            else reject sTAGE_FORMULA Big_int_Z.zero_big_int
-                   eRR_BAD_IMP_PAYLOAD
-       else reject sTAGE_FORMULA Big_int_Z.zero_big_int eRR_NOT_IMP
-  else reject sTAGE_FORMULA Big_int_Z.zero_big_int eRR_NONCANONICAL_FORMULA
 
 (** val parse_formula_diagnostic : Big_int_Z.big_int -> Big_int_Z.big_int **)
 
@@ -1531,309 +667,6 @@ let result_status =
 
 let result_payload =
   snd001
-
-(** val acceptedb : Big_int_Z.big_int -> bool **)
-
-let acceptedb r1 =
-  Nat.eqb (result_status r1) sTATUS_ACCEPT
-
-(** val parsed_line_formula : Big_int_Z.big_int -> Big_int_Z.big_int **)
-
-let parsed_line_formula =
-  snd001
-
-(** val nth_line :
-    Big_int_Z.big_int -> Big_int_Z.big_int -> Big_int_Z.big_int ->
-    Big_int_Z.big_int **)
-
-let nth_line n body i =
-  nth_list_fuel (Big_int_Z.succ_big_int n) body i
-
-(** val check_axk : Big_int_Z.big_int -> Big_int_Z.big_int **)
-
-let check_axk phi =
-  let outer = parse_imp phi in
-  if acceptedb outer
-  then let outer_payload = result_payload outer in
-       let a = fst001 outer_payload in
-       let rhs = snd001 outer_payload in
-       let inner = parse_imp rhs in
-       if acceptedb inner
-       then let inner_payload = result_payload inner in
-            let b0 = fst001 inner_payload in
-            let a2 = snd001 inner_payload in
-            if Nat.eqb a a2
-            then if is_formula a
-                 then if is_formula b0
-                      then accept (encode rULE_AXK (encode a b0))
-                      else reject sTAGE_RULE Big_int_Z.zero_big_int
-                             eRR_AXK_BAD_B
-                 else reject sTAGE_RULE Big_int_Z.zero_big_int eRR_AXK_BAD_A
-            else reject sTAGE_RULE Big_int_Z.zero_big_int eRR_AXK_A_MISMATCH
-       else reject sTAGE_RULE Big_int_Z.zero_big_int eRR_AXK_NOT_IMP_2
-  else reject sTAGE_RULE Big_int_Z.zero_big_int eRR_AXK_NOT_IMP_1
-
-(** val check_axs : Big_int_Z.big_int -> Big_int_Z.big_int **)
-
-let check_axs phi =
-  let imp1 = parse_imp phi in
-  if acceptedb imp1
-  then let p1 = result_payload imp1 in
-       let x = fst001 p1 in
-       let y = snd001 p1 in
-       let imp2 = parse_imp x in
-       if acceptedb imp2
-       then let p2 = result_payload imp2 in
-            let a = fst001 p2 in
-            let bC = snd001 p2 in
-            let imp3 = parse_imp bC in
-            if acceptedb imp3
-            then let p3 = result_payload imp3 in
-                 let b0 = fst001 p3 in
-                 let c = snd001 p3 in
-                 let imp4 = parse_imp y in
-                 if acceptedb imp4
-                 then let p4 = result_payload imp4 in
-                      let aB = fst001 p4 in
-                      let aC = snd001 p4 in
-                      let imp5 = parse_imp aB in
-                      if acceptedb imp5
-                      then let p5 = result_payload imp5 in
-                           let a1 = fst001 p5 in
-                           let b1 = snd001 p5 in
-                           let imp6 = parse_imp aC in
-                           if acceptedb imp6
-                           then let p6 = result_payload imp6 in
-                                let a2 = fst001 p6 in
-                                let c1 = snd001 p6 in
-                                if Nat.eqb a a1
-                                then if Nat.eqb a a2
-                                     then if Nat.eqb b0 b1
-                                          then if Nat.eqb c c1
-                                               then if is_formula a
-                                                    then if is_formula b0
-                                                         then if is_formula c
-                                                              then accept
-                                                                    (encode
-                                                                    rULE_AXS
-                                                                    (encode a
-                                                                    (encode
-                                                                    b0 c)))
-                                                              else reject
-                                                                    sTAGE_RULE
-                                                                    Big_int_Z.zero_big_int
-                                                                    eRR_AXS_BAD_C
-                                                         else reject
-                                                                sTAGE_RULE
-                                                                Big_int_Z.zero_big_int
-                                                                eRR_AXS_BAD_B
-                                                    else reject sTAGE_RULE
-                                                           Big_int_Z.zero_big_int
-                                                           eRR_AXS_BAD_A
-                                               else reject sTAGE_RULE
-                                                      Big_int_Z.zero_big_int
-                                                      eRR_AXS_C_MISMATCH
-                                          else reject sTAGE_RULE
-                                                 Big_int_Z.zero_big_int
-                                                 eRR_AXS_B_MISMATCH
-                                     else reject sTAGE_RULE
-                                            Big_int_Z.zero_big_int
-                                            eRR_AXS_A_MISMATCH_RIGHT
-                                else reject sTAGE_RULE Big_int_Z.zero_big_int
-                                       eRR_AXS_A_MISMATCH_LEFT
-                           else reject sTAGE_RULE Big_int_Z.zero_big_int
-                                  eRR_AXS_NOT_IMP_6
-                      else reject sTAGE_RULE Big_int_Z.zero_big_int
-                             eRR_AXS_NOT_IMP_5
-                 else reject sTAGE_RULE Big_int_Z.zero_big_int
-                        eRR_AXS_NOT_IMP_4
-            else reject sTAGE_RULE Big_int_Z.zero_big_int eRR_AXS_NOT_IMP_3
-       else reject sTAGE_RULE Big_int_Z.zero_big_int eRR_AXS_NOT_IMP_2
-  else reject sTAGE_RULE Big_int_Z.zero_big_int eRR_AXS_NOT_IMP_1
-
-(** val line_formula_result :
-    Big_int_Z.big_int -> Big_int_Z.big_int -> Big_int_Z.big_int ->
-    Big_int_Z.big_int -> Big_int_Z.big_int **)
-
-let line_formula_result n body i detail =
-  let fetched = nth_line n body i in
-  if acceptedb fetched
-  then let parsed = parse_line (result_payload fetched) in
-       if acceptedb parsed
-       then accept (parsed_line_formula (result_payload parsed))
-       else reject sTAGE_RULE i detail
-  else reject sTAGE_RULE i detail
-
-(** val check_mp :
-    Big_int_Z.big_int -> Big_int_Z.big_int -> Big_int_Z.big_int ->
-    Big_int_Z.big_int -> Big_int_Z.big_int -> Big_int_Z.big_int **)
-
-let check_mp n body j p q =
-  if Nat.ltb p j
-  then if Nat.ltb q j
-       then if Nat.ltb j n
-            then let rj = line_formula_result n body j eRR_MP_BAD_LINE_J in
-                 if acceptedb rj
-                 then let phi_j = result_payload rj in
-                      let rp = line_formula_result n body p eRR_MP_BAD_LINE_P
-                      in
-                      if acceptedb rp
-                      then let phi_p = result_payload rp in
-                           let rq =
-                             line_formula_result n body q eRR_MP_BAD_LINE_Q
-                           in
-                           if acceptedb rq
-                           then let phi_q = result_payload rq in
-                                let parsed_q = parse_imp phi_q in
-                                if acceptedb parsed_q
-                                then let q_payload = result_payload parsed_q
-                                     in
-                                     let a = fst001 q_payload in
-                                     let b0 = snd001 q_payload in
-                                     if Nat.eqb a phi_p
-                                     then if Nat.eqb b0 phi_j
-                                          then accept
-                                                 (encode rULE_MP
-                                                   (encode p
-                                                     (encode q (encode a b0))))
-                                          else reject sTAGE_RULE j
-                                                 eRR_MP_CONSEQUENT_MISMATCH
-                                     else reject sTAGE_RULE j
-                                            eRR_MP_ANTECEDENT_MISMATCH
-                                else reject sTAGE_RULE j eRR_MP_Q_NOT_IMP
-                           else reject sTAGE_RULE q eRR_MP_BAD_LINE_Q
-                      else reject sTAGE_RULE p eRR_MP_BAD_LINE_P
-                 else reject sTAGE_RULE j eRR_MP_BAD_LINE_J
-            else reject sTAGE_RULE j eRR_MP_BAD_LINE_J
-       else reject sTAGE_RULE j eRR_MP_Q_NOT_LT_J
-  else reject sTAGE_RULE j eRR_MP_P_NOT_LT_J
-
-(** val code_local_cert_payload :
-    Big_int_Z.big_int -> Big_int_Z.big_int -> Big_int_Z.big_int **)
-
-let code_local_cert_payload =
-  encode
-
-(** val code_final_cert_payload :
-    Big_int_Z.big_int -> Big_int_Z.big_int -> Big_int_Z.big_int ->
-    Big_int_Z.big_int -> Big_int_Z.big_int **)
-
-let code_final_cert_payload n theta certs final_formula =
-  encode n (encode theta (encode certs final_formula))
-
-(** val verify_line :
-    Big_int_Z.big_int -> Big_int_Z.big_int -> Big_int_Z.big_int ->
-    Big_int_Z.big_int **)
-
-let verify_line n body j =
-  let fetched = nth_line n body j in
-  if acceptedb fetched
-  then let ell = result_payload fetched in
-       if canonical001b ell
-       then let tag = line_tag ell in
-            let phi = line_formula ell in
-            let parsed_tag = parse_rule_tag tag in
-            if acceptedb parsed_tag
-            then let tag_payload = result_payload parsed_tag in
-                 let rule = fst001 tag_payload in
-                 let payload = snd001 tag_payload in
-                 if Nat.eqb rule rULE_AXK
-                 then let checked = check_axk phi in
-                      if acceptedb checked
-                      then accept
-                             (code_local_cert_payload j
-                               (result_payload checked))
-                      else reject sTAGE_RULE j (result_payload checked)
-                 else if Nat.eqb rule rULE_AXS
-                      then let checked = check_axs phi in
-                           if acceptedb checked
-                           then accept
-                                  (code_local_cert_payload j
-                                    (result_payload checked))
-                           else reject sTAGE_RULE j (result_payload checked)
-                      else if Nat.eqb rule rULE_MP
-                           then if canonical001b payload
-                                then let p = fst001 payload in
-                                     let q = snd001 payload in
-                                     let checked = check_mp n body j p q in
-                                     if acceptedb checked
-                                     then accept
-                                            (code_local_cert_payload j
-                                              (result_payload checked))
-                                     else reject sTAGE_RULE j
-                                            (result_payload checked)
-                                else reject sTAGE_TAG j eRR_NONCANONICAL_NODE
-                           else reject sTAGE_TAG j eRR_UNKNOWN_RULE
-            else reject sTAGE_TAG j (result_payload parsed_tag)
-       else reject sTAGE_LINE j eRR_NONCANONICAL_LINE
-  else reject sTAGE_LINE j (result_payload fetched)
-
-(** val verify_lines :
-    Big_int_Z.big_int -> Big_int_Z.big_int -> Big_int_Z.big_int ->
-    Big_int_Z.big_int -> Big_int_Z.big_int -> Big_int_Z.big_int **)
-
-let rec verify_lines fuel n body j certs =
-  (fun fO fS n -> if Big_int_Z.sign_big_int n <= 0 then fO ()
-  else fS (Big_int_Z.pred_big_int n))
-    (fun _ ->
-    if Nat.eqb j n
-    then accept certs
-    else reject sTAGE_RULE j eRR_FUEL_EXHAUSTED)
-    (fun fuel' ->
-    if Nat.eqb j n
-    then accept certs
-    else let checked = verify_line n body j in
-         if acceptedb checked
-         then let local_cert = result_payload checked in
-              verify_lines fuel' n body (Big_int_Z.succ_big_int j)
-                (code_cons local_cert certs)
-         else checked)
-    fuel
-
-(** val final_formula_result :
-    Big_int_Z.big_int -> Big_int_Z.big_int -> Big_int_Z.big_int **)
-
-let final_formula_result n body =
-  let last = Nat.pred n in
-  let fetched = nth_line n body last in
-  if acceptedb fetched
-  then let parsed = parse_line (result_payload fetched) in
-       if acceptedb parsed
-       then accept (parsed_line_formula (result_payload parsed))
-       else reject sTAGE_CONCLUSION last (result_payload parsed)
-  else reject sTAGE_CONCLUSION last (result_payload fetched)
-
-(** val a002_Verify :
-    Big_int_Z.big_int -> Big_int_Z.big_int -> Big_int_Z.big_int **)
-
-let a002_Verify d theta =
-  if canonical001b d
-  then let n = fst001 d in
-       let body = snd001 d in
-       if list_exact_lengthb n body
-       then if Nat.eqb n Big_int_Z.zero_big_int
-            then reject sTAGE_CONCLUSION Big_int_Z.zero_big_int
-                   eRR_EMPTY_DERIVATION
-            else let checked_lines =
-                   verify_lines n n body Big_int_Z.zero_big_int code_nil
-                 in
-                 if acceptedb checked_lines
-                 then let certs = result_payload checked_lines in
-                      let final_formula = final_formula_result n body in
-                      if acceptedb final_formula
-                      then let phi_last = result_payload final_formula in
-                           if Nat.eqb phi_last theta
-                           then accept
-                                  (code_final_cert_payload n theta certs
-                                    phi_last)
-                           else reject sTAGE_CONCLUSION (Nat.pred n)
-                                  eRR_BAD_CONCLUSION
-                      else final_formula
-                 else checked_lines
-       else reject sTAGE_LIST_STRUCTURE Big_int_Z.zero_big_int
-              eRR_BAD_DERIVATION_LENGTH
-  else reject sTAGE_DERIVATION_HEADER Big_int_Z.zero_big_int
-         eRR_NONCANONICAL_DERIVATION
 
 type normalizedFormula =
 | NFVar of Big_int_Z.big_int
@@ -1973,7 +806,9 @@ let rec normalize_formula_fuel fuel c =
 (** val normalize_formula : Big_int_Z.big_int -> normalizedFormula option **)
 
 let normalize_formula c =
-  normalize_formula_fuel (formula_bound c) c
+  if canonical001b c
+  then normalize_formula_fuel (fst001 c) (snd001 c)
+  else None
 
 (** val normalize_rule : Big_int_Z.big_int -> normalizedRule option **)
 
@@ -2039,6 +874,39 @@ let rec normalize_lines n body =
 let normalize_derivation d =
   if canonical001b d then normalize_lines (fst001 d) (snd001 d) else None
 
+(** val normalized_failure_index :
+    normalizedFormula list -> normalizedDerivation -> Big_int_Z.big_int ->
+    Big_int_Z.big_int option **)
+
+let rec normalized_failure_index prefix lines index =
+  match lines with
+  | [] -> None
+  | line :: rest ->
+    if normalized_stepb prefix line.normalized_line_rule
+         line.normalized_line_formula
+    then normalized_failure_index
+           (app prefix (line.normalized_line_formula :: [])) rest
+           (Big_int_Z.succ_big_int index)
+    else Some index
+
+(** val normalized_rejection : normalizedDerivation -> Big_int_Z.big_int **)
+
+let normalized_rejection lines =
+  match normalized_failure_index [] lines Big_int_Z.zero_big_int with
+  | Some index -> reject sTAGE_RULE index eRR_NORMALIZED_STEP_REJECTED
+  | None ->
+    (match normalized_conclusion lines with
+     | Some _ ->
+       reject sTAGE_CONCLUSION (Nat.pred (length lines)) eRR_BAD_CONCLUSION
+     | None ->
+       reject sTAGE_CONCLUSION Big_int_Z.zero_big_int eRR_EMPTY_DERIVATION)
+
+(** val certified_payload :
+    Big_int_Z.big_int -> Big_int_Z.big_int -> Big_int_Z.big_int **)
+
+let certified_payload =
+  encode
+
 (** val a002_Verify_certified :
     Big_int_Z.big_int -> Big_int_Z.big_int -> Big_int_Z.big_int **)
 
@@ -2048,11 +916,10 @@ let a002_Verify_certified d theta =
     (match normalize_formula theta with
      | Some target ->
        if normalized_verifyb lines target
-       then a002_Verify d theta
-       else reject sTAGE_RULE Big_int_Z.zero_big_int eRR_BAD_CONCLUSION
+       then accept (certified_payload d theta)
+       else normalized_rejection lines
      | None ->
-       reject sTAGE_DERIVATION_HEADER Big_int_Z.zero_big_int
-         eRR_NONCANONICAL_DERIVATION)
+       reject sTAGE_FORMULA Big_int_Z.zero_big_int eRR_NONCANONICAL_FORMULA)
   | None ->
     reject sTAGE_DERIVATION_HEADER Big_int_Z.zero_big_int
       eRR_NONCANONICAL_DERIVATION
@@ -2061,7 +928,15 @@ let a002_Verify_certified d theta =
     Big_int_Z.big_int -> Big_int_Z.big_int -> Big_int_Z.big_int -> bool **)
 
 let a002_Certified_Certb d theta payload =
-  Nat.eqb (a002_Verify_certified d theta) (accept payload)
+  (&&)
+    ((&&) ((&&) (canonical001b payload) (Nat.eqb (fst001 payload) d))
+      (Nat.eqb (snd001 payload) theta))
+    (match normalize_derivation d with
+     | Some lines ->
+       (match normalize_formula theta with
+        | Some target -> normalized_verifyb lines target
+        | None -> false)
+     | None -> false)
 
 type a002_IO_Query =
 | Verify_Query of Big_int_Z.big_int * Big_int_Z.big_int
