theories/A002/_appendix/_artifacts/A002_IO.mli
@@ -5,6 +5,8 @@ val fst : ('a1 * 'a2) -> 'a1
 
 val snd : ('a1 * 'a2) -> 'a2
 
+val length : 'a1 list -> Big_int_Z.big_int
+
 val app : 'a1 list -> 'a1 list -> 'a1 list
 
 val add : Big_int_Z.big_int -> Big_int_Z.big_int -> Big_int_Z.big_int
@@ -139,8 +141,6 @@ val reject :
 
 val sTAGE_DERIVATION_HEADER : Big_int_Z.big_int
 
-val sTAGE_LIST_STRUCTURE : Big_int_Z.big_int
-
 val sTAGE_LINE : Big_int_Z.big_int
 
 val sTAGE_TAG : Big_int_Z.big_int
@@ -153,85 +153,23 @@ val sTAGE_CONCLUSION : Big_int_Z.big_int
 
 val eRR_NONCANONICAL_DERIVATION : Big_int_Z.big_int
 
-val eRR_BAD_DERIVATION_LENGTH : Big_int_Z.big_int
-
 val eRR_EMPTY_DERIVATION : Big_int_Z.big_int
 
 val eRR_BAD_CONCLUSION : Big_int_Z.big_int
-
-val eRR_FUEL_EXHAUSTED : Big_int_Z.big_int
 
 val eRR_NONCANONICAL_NODE : Big_int_Z.big_int
 
 val eRR_BAD_TAG : Big_int_Z.big_int
 
-val eRR_BAD_LIST_TAG : Big_int_Z.big_int
-
-val eRR_INDEX_OUT_OF_RANGE : Big_int_Z.big_int
-
 val eRR_NONCANONICAL_LINE : Big_int_Z.big_int
 
 val eRR_UNKNOWN_RULE : Big_int_Z.big_int
 
+val eRR_NORMALIZED_STEP_REJECTED : Big_int_Z.big_int
+
 val eRR_NONCANONICAL_FORMULA : Big_int_Z.big_int
 
 val eRR_BAD_FORMULA_TAG : Big_int_Z.big_int
-
-val eRR_BAD_IMP_PAYLOAD : Big_int_Z.big_int
-
-val eRR_NOT_IMP : Big_int_Z.big_int
-
-val eRR_AXK_NOT_IMP_1 : Big_int_Z.big_int
-
-val eRR_AXK_NOT_IMP_2 : Big_int_Z.big_int
-
-val eRR_AXK_A_MISMATCH : Big_int_Z.big_int
-
-val eRR_AXK_BAD_A : Big_int_Z.big_int
-
-val eRR_AXK_BAD_B : Big_int_Z.big_int
-
-val eRR_AXS_NOT_IMP_1 : Big_int_Z.big_int
-
-val eRR_AXS_NOT_IMP_2 : Big_int_Z.big_int
-
-val eRR_AXS_NOT_IMP_3 : Big_int_Z.big_int
-
-val eRR_AXS_NOT_IMP_4 : Big_int_Z.big_int
-
-val eRR_AXS_NOT_IMP_5 : Big_int_Z.big_int
-
-val eRR_AXS_NOT_IMP_6 : Big_int_Z.big_int
-
-val eRR_AXS_A_MISMATCH_LEFT : Big_int_Z.big_int
-
-val eRR_AXS_A_MISMATCH_RIGHT : Big_int_Z.big_int
-
-val eRR_AXS_B_MISMATCH : Big_int_Z.big_int
-
-val eRR_AXS_C_MISMATCH : Big_int_Z.big_int
-
-val eRR_AXS_BAD_A : Big_int_Z.big_int
-
-val eRR_AXS_BAD_B : Big_int_Z.big_int
-
-val eRR_AXS_BAD_C : Big_int_Z.big_int
-
-val eRR_MP_P_NOT_LT_J : Big_int_Z.big_int
-
-val eRR_MP_Q_NOT_LT_J : Big_int_Z.big_int
-
-val eRR_MP_BAD_LINE_J : Big_int_Z.big_int
-
-val eRR_MP_BAD_LINE_P : Big_int_Z.big_int
-
-val eRR_MP_BAD_LINE_Q : Big_int_Z.big_int
-
-val eRR_MP_Q_NOT_IMP : Big_int_Z.big_int
-
-val eRR_MP_ANTECEDENT_MISMATCH : Big_int_Z.big_int
-
-val eRR_MP_CONSEQUENT_MISMATCH : Big_int_Z.big_int
 
 val fst001 : Big_int_Z.big_int -> Big_int_Z.big_int
 
@@ -248,23 +186,11 @@ val tAG_NIL : Big_int_Z.big_int
 
 val tAG_CONS : Big_int_Z.big_int
 
-val code_nil : Big_int_Z.big_int
-
-val code_cons : Big_int_Z.big_int -> Big_int_Z.big_int -> Big_int_Z.big_int
-
 val list_tag : Big_int_Z.big_int -> Big_int_Z.big_int
 
 val list_payload : Big_int_Z.big_int -> Big_int_Z.big_int
 
 val is_nil_nodeb : Big_int_Z.big_int -> bool
-
-val cons_payloadb : Big_int_Z.big_int -> bool
-
-val list_exact_lengthb : Big_int_Z.big_int -> Big_int_Z.big_int -> bool
-
-val nth_list_fuel :
-  Big_int_Z.big_int -> Big_int_Z.big_int -> Big_int_Z.big_int ->
-  Big_int_Z.big_int
 
 val tAG_VAR : Big_int_Z.big_int
 
@@ -279,8 +205,6 @@ val is_formula_fuel : Big_int_Z.big_int -> Big_int_Z.big_int -> bool
 val formula_bound : Big_int_Z.big_int -> Big_int_Z.big_int
 
 val is_formula : Big_int_Z.big_int -> bool
-
-val parse_imp : Big_int_Z.big_int -> Big_int_Z.big_int
 
 val parse_formula_diagnostic : Big_int_Z.big_int -> Big_int_Z.big_int
 
@@ -305,46 +229,6 @@ val parse_line : Big_int_Z.big_int -> Big_int_Z.big_int
 val result_status : Big_int_Z.big_int -> Big_int_Z.big_int
 
 val result_payload : Big_int_Z.big_int -> Big_int_Z.big_int
-
-val acceptedb : Big_int_Z.big_int -> bool
-
-val parsed_line_formula : Big_int_Z.big_int -> Big_int_Z.big_int
-
-val nth_line :
-  Big_int_Z.big_int -> Big_int_Z.big_int -> Big_int_Z.big_int ->
-  Big_int_Z.big_int
-
-val check_axk : Big_int_Z.big_int -> Big_int_Z.big_int
-
-val check_axs : Big_int_Z.big_int -> Big_int_Z.big_int
-
-val line_formula_result :
-  Big_int_Z.big_int -> Big_int_Z.big_int -> Big_int_Z.big_int ->
-  Big_int_Z.big_int -> Big_int_Z.big_int
-
-val check_mp :
-  Big_int_Z.big_int -> Big_int_Z.big_int -> Big_int_Z.big_int ->
-  Big_int_Z.big_int -> Big_int_Z.big_int -> Big_int_Z.big_int
-
-val code_local_cert_payload :
-  Big_int_Z.big_int -> Big_int_Z.big_int -> Big_int_Z.big_int
-
-val code_final_cert_payload :
-  Big_int_Z.big_int -> Big_int_Z.big_int -> Big_int_Z.big_int ->
-  Big_int_Z.big_int -> Big_int_Z.big_int
-
-val verify_line :
-  Big_int_Z.big_int -> Big_int_Z.big_int -> Big_int_Z.big_int ->
-  Big_int_Z.big_int
-
-val verify_lines :
-  Big_int_Z.big_int -> Big_int_Z.big_int -> Big_int_Z.big_int ->
-  Big_int_Z.big_int -> Big_int_Z.big_int -> Big_int_Z.big_int
-
-val final_formula_result :
-  Big_int_Z.big_int -> Big_int_Z.big_int -> Big_int_Z.big_int
-
-val a002_Verify : Big_int_Z.big_int -> Big_int_Z.big_int -> Big_int_Z.big_int
 
 type normalizedFormula =
 | NFVar of Big_int_Z.big_int
@@ -384,6 +268,15 @@ val normalize_lines :
   Big_int_Z.big_int -> Big_int_Z.big_int -> normalizedDerivation option
 
 val normalize_derivation : Big_int_Z.big_int -> normalizedDerivation option
+
+val normalized_failure_index :
+  normalizedFormula list -> normalizedDerivation -> Big_int_Z.big_int ->
+  Big_int_Z.big_int option
+
+val normalized_rejection : normalizedDerivation -> Big_int_Z.big_int
+
+val certified_payload :
+  Big_int_Z.big_int -> Big_int_Z.big_int -> Big_int_Z.big_int
 
 val a002_Verify_certified :
   Big_int_Z.big_int -> Big_int_Z.big_int -> Big_int_Z.big_int
